Cofinite.v
@@ -1,0 +1,1561 @@
+(************************************************
+ *          Row Subtyping - Cofinite            *
+ *                 Leo White                    *
+ ************************************************)
+
+Set Implicit Arguments.
+
+Require Import MSets.
+Require Import MSetList.
+Require Import Arith.
+
+(**************************************************************)
+(* CSet                                                       *)
+(**************************************************************)
+
+Module CSet.
+
+  Module E <: OrderedTypeWithLeibniz.
+    Include PeanoNat.Nat.
+    Definition eq_leibniz a b (H:eq a b) := H.
+  End E.
+
+  Module MSet := MakeWithLeibniz(E).
+
+  Module MSetFacts := Facts(MSet).
+
+  Module MSetProperties := Properties(MSet).
+
+  Module MSetEqProperties := EqProperties(MSet).
+
+  Module MSetDecide := Decide(MSet).
+
+  Definition elt := nat.
+
+  Inductive t : Type :=
+    | finite : MSet.t -> t
+    | cofinite : MSet.t -> t.
+
+  Definition empty := finite MSet.empty.
+
+  Definition is_empty cs :=
+    match cs with
+    | finite ms => MSet.is_empty ms
+    | cofinite _ => false
+    end.
+
+  Definition universe := cofinite MSet.empty.
+
+  Definition is_universe cs :=
+    match cs with
+    | finite _ => false
+    | cofinite ms => MSet.is_empty ms
+    end.
+
+  Definition mem x cs :=
+    match cs with
+    | finite ms => MSet.mem x ms
+    | cofinite ms => negb (MSet.mem x ms)
+    end.
+
+  Definition add x cs :=
+    match cs with
+    | finite ms => finite (MSet.add x ms)
+    | cofinite ms => cofinite (MSet.remove x ms)
+    end. 
+
+  Definition singleton x :=
+    finite (MSet.singleton x).
+
+  Definition cosingleton x :=
+    cofinite (MSet.singleton x).
+
+  Definition remove x cs :=
+    match cs with
+    | finite ms => finite (MSet.remove x ms)
+    | cofinite ms => cofinite (MSet.add x ms)
+    end. 
+
+  Definition union cs1 cs2 :=
+    match cs1, cs2 with
+    | finite ms1, finite ms2 => finite (MSet.union ms1 ms2)
+    | finite ms1, cofinite ms2 => cofinite (MSet.diff ms2 ms1)
+    | cofinite ms1, finite ms2 => cofinite (MSet.diff ms1 ms2)
+    | cofinite ms1, cofinite ms2 => cofinite (MSet.inter ms1 ms2)
+    end.
+
+  Definition inter cs1 cs2 := 
+    match cs1, cs2 with
+    | finite ms1, finite ms2 => finite (MSet.inter ms1 ms2)
+    | finite ms1, cofinite ms2 => finite (MSet.diff ms1 ms2)
+    | cofinite ms1, finite ms2 => finite (MSet.diff ms2 ms1)
+    | cofinite ms1, cofinite ms2 => cofinite (MSet.union ms1 ms2)
+    end.
+
+  Definition diff cs1 cs2 := 
+    match cs1, cs2 with
+    | finite ms1, finite ms2 => finite (MSet.diff ms1 ms2)
+    | finite ms1, cofinite ms2 => finite (MSet.inter ms1 ms2)
+    | cofinite ms1, finite ms2 => cofinite (MSet.union ms1 ms2)
+    | cofinite ms1, cofinite ms2 => finite (MSet.diff ms2 ms1)
+    end.
+
+  Definition equal cs1 cs2 :=
+    match cs1, cs2 with
+    | finite ms1, finite ms2 => MSet.equal ms1 ms2
+    | finite _, cofinite _ => false
+    | cofinite _, finite _ => false
+    | cofinite ms1, cofinite ms2 => MSet.equal ms1 ms2
+    end.
+
+  Definition subset cs1 cs2 :=
+    match cs1, cs2 with
+    | finite ms1, finite ms2 => MSet.subset ms1 ms2
+    | finite ms1, cofinite ms2 => MSet.is_empty (MSet.inter ms1 ms2)
+    | cofinite ms1, finite ms2 => false
+    | cofinite ms1, cofinite ms2 => MSet.subset ms2 ms1
+    end.
+
+  Definition disjoint cs1 cs2 :=
+    is_empty (inter cs1 cs2).
+
+  Local Definition not_in_mset ms :=
+    match MSet.max_elt ms with
+    | None => 0
+    | Some max => S max
+    end.
+
+  Definition choose cs :=
+    match cs with
+    | finite ms => MSet.choose ms
+    | cofinite ms => Some (not_in_mset ms)
+    end.
+
+  (** Return one element of the given set, or [None] if
+  the set is empty. Which element is chosen is unspecified.
+  Equal sets could return different elements. *)
+
+  Definition In x cs :=
+    match cs with
+    | finite ms => MSet.In x ms
+    | cofinite ms => not (MSet.In x ms)
+    end.
+
+  Definition Equal cs1 cs2 := forall x : elt, In x cs1 <-> In x cs2.
+
+  Definition Subset cs1 cs2 := forall x : elt, In x cs1 -> In x cs2.
+
+  Definition Empty cs := forall x : elt, ~ In x cs.
+
+  Definition Universe cs := forall x : elt, In x cs.
+
+  Definition For_all (P : elt -> Prop) cs := forall x, In x cs -> P x.
+
+  Definition Exists (P : elt -> Prop) cs := exists x, In x cs /\ P x.
+
+  Definition Disjoint cs1 cs2 :=
+    forall x : elt, In x cs1 -> ~ In x cs2.
+
+  Definition eq : t -> t -> Prop := Equal.
+
+  Local Lemma not_in_mset_spec : forall ms,
+    not (MSet.In (not_in_mset ms) ms).
+  Proof.
+    intro ms.
+    unfold not_in_mset.
+    remember (MSet.max_elt ms) as max.
+    destruct max as [max | ].
+    - intro H.
+      apply MSet.max_elt_spec2 with (x := max) in H; auto.
+    - apply MSet.max_elt_spec3.
+      auto.
+  Qed.
+
+  Local Lemma choose_not_in_mset : forall ms,
+    exists x : elt, not (MSet.In x ms).
+  Proof.
+    intro ms.
+    exists (x := not_in_mset ms).
+    apply not_in_mset_spec.
+  Qed.
+
+  Local Lemma not_not_in_to_in : forall ms1 ms2,
+      ~ (forall x : elt, ~ MSet.In x ms2 -> MSet.In x ms1).
+  Proof.
+    intros ms1 ms2 Hto.
+    destruct (choose_not_in_mset (MSet.union ms1 ms2)) as [x Hnot].
+    rewrite MSet.union_spec in Hnot.
+    assert (~ MSet.In x ms1) as Hnot1 by intuition auto.
+    assert (~ MSet.In x ms2) as Hnot2 by intuition auto.
+    apply Hto in Hnot2.
+    auto.
+  Qed.
+
+  Local Lemma not_in_iff_not_in : forall ms1 ms2,
+      ~ (forall x : elt, MSet.In x ms1 <-> ~ MSet.In x ms2).
+  Proof.
+    intros ms1 ms2 Hiff.
+    apply (@not_not_in_to_in ms1 ms2).
+    intro x.
+    destruct (Hiff x).
+    assumption.
+  Qed.
+
+  Local Lemma not_not_in_iff_in : forall ms1 ms2,
+      ~ (forall x : elt, ~ MSet.In x ms1 <-> MSet.In x ms2).
+  Proof.
+    intros ms1 ms2 H.
+    apply not_in_iff_not_in with (ms1 := ms2) (ms2 := ms1).
+    firstorder.
+  Qed.
+
+  Local Lemma eq_not_in : forall ms1 ms2,
+      MSet.eq ms1 ms2 <->
+      forall x : elt, ~ MSet.In x ms1 <-> ~ MSet.In x ms2.
+  Proof.
+    intros ms1 ms2.
+    split.
+    - intro Heq.
+      split; intro Hnot.
+      + rewrite Heq in Hnot.
+        auto.
+      + rewrite <- Heq in Hnot.
+        auto.
+    - intro Hiff.
+      split; intro Hin.
+      + destruct (MSetProperties.In_dec a ms2) as [Hin2 | Hnot2];
+          auto.
+        rewrite <- Hiff in Hnot2.
+        exfalso; auto.
+      + destruct (MSetProperties.In_dec a ms1) as [Hin2 | Hnot2];
+          auto.
+        rewrite Hiff in Hnot2.
+        exfalso; auto.
+  Qed.
+
+  Lemma eq_leibniz : forall cs1 cs2,
+      eq cs1 cs2 -> cs1 = cs2.
+  Proof.
+    unfold eq.
+    intros cs1 cs2.
+    destruct cs1 as [ms1 | ms1]; destruct cs2 as [ms2 | ms2];
+      unfold Equal, In; intro H.
+    - f_equal; apply MSet.eq_leibniz; auto.
+    - exfalso.
+      apply not_in_iff_not_in with (ms1 := ms1) (ms2 := ms2).
+      auto.
+    - exfalso.
+      apply not_not_in_iff_in with (ms1 := ms1) (ms2 := ms2).
+      auto.
+    - f_equal. apply MSet.eq_leibniz.
+      rewrite eq_not_in.
+      auto.
+  Qed.
+
+  Instance Equal_equiv :
+    Equivalence Equal.
+  Proof.  
+    firstorder.
+  Qed.
+
+  Lemma eq_dec :
+    forall cs1 cs2, { eq cs1 cs2 } + { ~ eq cs1 cs2 }.
+  Proof.
+    intros cs1 cs2.
+    destruct cs1 as [ms1 | ms1]; destruct cs2 as [ms2 | ms2];
+      unfold eq, Equal, In.
+    - destruct MSet.eq_dec with (s := ms1) (s' := ms2); auto.
+    - right.
+      apply not_in_iff_not_in.
+    - right.
+      apply not_not_in_iff_in.
+    - destruct MSet.eq_dec with (s := ms1) (s' := ms2).
+      + left.
+        rewrite <- eq_not_in.      
+        auto.
+      + right.
+        rewrite <- eq_not_in.
+        auto.
+  Qed.
+
+  Section Spec.
+    Variable cs cs1 cs2: t.
+    Variable x y : elt.
+
+    Lemma mem_spec:
+      mem x cs = true <-> In x cs.
+    Proof.
+      destruct cs as [ms | ms];
+        unfold mem, In; rewrite <- MSet.mem_spec.
+      - reflexivity.
+      - rewrite negb_true_iff.
+        rewrite Bool.not_true_iff_false.
+        reflexivity.
+    Qed.
+
+    Lemma equal_spec :
+      equal cs1 cs2 = true <-> Equal cs1 cs2.
+    Proof.
+      destruct cs1 as [ms1 | ms1]; destruct cs2 as [ms2 | ms2];
+        unfold equal, Equal, In.
+      - rewrite MSet.equal_spec.
+        unfold MSet.Equal.
+        reflexivity.
+      - split.
+        + discriminate.
+        + intro Heq.
+          exfalso.
+          apply not_in_iff_not_in in Heq.
+          assumption.
+      - split.
+        + discriminate.
+        + intro Heq.
+          exfalso.
+          apply not_not_in_iff_in in Heq.
+          assumption.
+      - rewrite MSet.equal_spec.
+        apply eq_not_in.
+    Qed.
+    
+    Lemma subset_spec :
+        subset cs1 cs2 = true <-> Subset cs1 cs2.
+    Proof.
+      clear cs.
+      destruct cs1 as [ms1 | ms1]; destruct cs2 as [ms2 | ms2];
+        unfold subset, Subset, In.
+      - rewrite MSet.subset_spec.
+        unfold MSet.Subset.
+        reflexivity.
+      - rewrite MSet.is_empty_spec.
+        unfold MSet.Empty.
+        split; intros H z.
+        + specialize H with (a := z).
+          rewrite MSet.inter_spec in H.
+          firstorder.
+        + rewrite MSet.inter_spec.
+          firstorder.
+      - split; intro H.
+        + discriminate.
+        + exfalso.
+          apply (@not_not_in_to_in ms2 ms1).
+          assumption.
+      - rewrite MSet.subset_spec.
+        unfold MSet.Subset.
+        split; intros Hto z Hin.
+        + auto.
+        + destruct (MSetProperties.In_dec z ms1) as [? | Hnotin];
+            auto.
+          apply Hto in Hnotin.
+          exfalso.
+          auto.
+    Qed.
+
+    Lemma empty_spec :
+      Empty empty.
+    Proof.
+      unfold empty, Empty, In.
+      MSetDecide.fsetdec.
+    Qed.
+
+    Lemma universe_spec :
+      Universe universe.
+    Proof.
+      unfold universe, Universe, In.
+      MSetDecide.fsetdec.
+    Qed.
+
+    Lemma is_empty_spec :
+      is_empty cs = true <-> Empty cs.
+    Proof.
+      destruct cs as [ms | ms]; unfold is_empty, Empty, In.
+      - rewrite MSet.is_empty_spec.
+        unfold MSet.Empty.
+        reflexivity.
+      - split; intro H.
+        + discriminate.
+        + exfalso.
+          destruct (choose_not_in_mset ms) as [z Hnotin].
+          apply (H z).
+          assumption.
+    Qed.
+
+    Lemma is_universe_spec :
+      is_universe cs = true <-> Universe cs.
+    Proof.
+      destruct cs as [ms | ms]; unfold is_universe, Universe, In.
+      - split; intro H.
+        + discriminate.
+        + exfalso.
+          destruct (choose_not_in_mset ms) as [z Hnotin].
+          apply Hnotin.
+          apply H.
+      - rewrite MSet.is_empty_spec.
+        unfold MSet.Empty.
+        reflexivity.
+    Qed.
+
+    Lemma add_spec :
+      In y (add x cs) <-> y = x \/ In y cs.
+    Proof.
+      destruct cs as [ms | ms]; unfold add, In;
+        split; MSetDecide.fsetdec.
+    Qed.      
+
+    Lemma remove_spec :
+        In y (remove x cs) <-> In y cs /\ y <> x.
+    Proof.
+      destruct cs as [ms | ms]; unfold remove, In;
+        split; MSetDecide.fsetdec.
+    Qed.      
+
+    Lemma singleton_spec :
+        In y (singleton x) <-> y = x.
+    Proof.
+      unfold In, singleton.
+      split; MSetDecide.fsetdec.
+    Qed.
+
+    Lemma cosingleton_spec :
+        ~ In y (cosingleton x) <-> y = x.
+    Proof.
+      unfold In, cosingleton.
+      split; MSetDecide.fsetdec.
+    Qed.
+
+    Lemma union_spec :
+      In x (union cs1 cs2) <-> In x cs1 \/ In x cs2.
+    Proof.
+      destruct cs1 as [ms1 | ms1]; destruct cs2 as [ms2 | ms2];
+        unfold union, In; split; MSetDecide.fsetdec.
+    Qed.
+
+    Lemma inter_spec :
+        In x (inter cs1 cs2) <-> In x cs1 /\ In x cs2.
+    Proof.
+      destruct cs1 as [ms1 | ms1]; destruct cs2 as [ms2 | ms2];
+        unfold inter, In; split; MSetDecide.fsetdec.
+    Qed.
+
+    Lemma diff_spec :
+      In x (diff cs1 cs2) <-> In x cs1 /\ ~In x cs2.
+    Proof.
+      destruct cs1 as [ms1 | ms1]; destruct cs2 as [ms2 | ms2];
+        unfold diff, In; split; MSetDecide.fsetdec.
+    Qed.
+
+    Lemma disjoint_spec :
+        disjoint cs1 cs2 = true <-> Disjoint cs1 cs2.
+    Proof.
+      destruct cs1 as [ms1 | ms1]; destruct cs2 as [ms2 | ms2];
+        unfold disjoint, is_empty, inter, Disjoint, In.
+      - rewrite MSet.is_empty_spec.
+        split. 
+        + MSetDecide.fsetdec.
+        + unfold MSet.Empty.
+          intros H z.
+          specialize H with (x := z).
+          MSetDecide.fsetdec.
+      - rewrite MSet.is_empty_spec.
+        split.
+        + MSetDecide.fsetdec. 
+        + unfold MSet.Empty.
+          intros H z.
+          specialize H with (x := z).
+          MSetDecide.fsetdec.
+      - rewrite MSet.is_empty_spec.
+        split.
+        + MSetDecide.fsetdec.
+        + unfold MSet.Empty.
+          intros H z.
+          specialize H with (x := z).
+          MSetDecide.fsetdec.
+      - split.
+        + intro.
+          discriminate.
+        + intro H.
+          exfalso.
+          apply (@not_not_in_to_in ms2 ms1).
+          intros z Hin1.
+          specialize H with (x := z).
+          destruct (MSetProperties.In_dec z ms2) as [? | Hnotin2];
+            auto.
+          exfalso.
+          apply H; auto.
+    Qed.
+
+    Lemma choose_spec1 :
+        choose cs = Some x -> In x cs.
+    Proof.
+      destruct cs as [ms | ms];
+        unfold choose, In.
+      - apply MSet.choose_spec1.
+      - intro H.
+        inversion H.
+        apply not_in_mset_spec.
+    Qed.      
+
+    Lemma choose_spec2 :
+        choose cs = None -> Empty cs.
+    Proof.
+      destruct cs as [ms | ms];
+        unfold choose, Empty, In.
+      - intro H.
+        apply MSet.choose_spec2 in H.
+        MSetDecide.fsetdec.
+      - intro.
+        discriminate.
+    Qed.
+
+  End Spec.
+
+End CSet.
+
+Import CSet.
+
+Definition cset := CSet.t.
+
+(**************************************************************)
+(* CSetFacts                                                  *)
+(**************************************************************)
+
+Module CSetFacts.
+
+  Notation eq_dec := E.eq_dec.
+  Definition eqb x y := if eq_dec x y then true else false.
+
+  Section ImplSpec.
+    Variable cs cs1 cs2 : t.
+    Variable x y : elt.
+
+    Lemma In_1 : E.eq x y -> In x cs -> In y cs.
+    Proof. intros E; rewrite E; auto. Qed.
+
+    Lemma mem_1 : In x cs -> mem x cs = true.
+    Proof. intros; apply <- mem_spec; auto. Qed.
+    Lemma mem_2 : mem x cs = true -> In x cs.
+    Proof. intros; apply -> mem_spec; auto. Qed.
+
+    Lemma equal_1 : Equal cs1 cs2 -> equal cs1 cs2 = true.
+    Proof. intros; apply <- equal_spec; auto. Qed.
+    Lemma equal_2 : equal cs1 cs2 = true -> Equal cs1 cs2.
+    Proof. intros; apply -> equal_spec; auto. Qed.
+
+    Lemma subset_1 : Subset cs1 cs2 -> subset cs1 cs2 = true.
+    Proof. intros; apply <- subset_spec; auto. Qed.
+    Lemma subset_2 : subset cs1 cs2 = true -> Subset cs1 cs2.
+    Proof. intros; apply -> subset_spec; auto. Qed.
+
+    Lemma is_empty_1 : Empty cs -> is_empty cs = true.
+    Proof. intros; apply <- is_empty_spec; auto. Qed.
+    Lemma is_empty_2 : is_empty cs = true -> Empty cs.
+    Proof. intros; apply -> is_empty_spec; auto. Qed.
+
+    Lemma is_universe_1 : Universe cs -> is_universe cs = true.
+    Proof. intros; apply <- is_universe_spec; auto. Qed.
+    Lemma is_universe_2 : is_universe cs = true -> Universe cs.
+    Proof. intros; apply -> is_universe_spec; auto. Qed.
+
+    Lemma add_1 : E.eq x y -> In y (add x cs).
+    Proof. intros; apply <- add_spec. auto with relations. Qed.
+    Lemma add_2 : In y cs -> In y (add x cs).
+    Proof. intros; apply <- add_spec; auto. Qed.
+    Lemma add_3 : ~ E.eq x y -> In y (add x cs) -> In y cs.
+    Proof.
+      rewrite add_spec. intros H [H'|H']; auto.
+      elim H; auto with relations.
+    Qed.
+    
+    Lemma remove_1 : E.eq x y -> ~ In y (remove x cs).
+    Proof. intros; rewrite remove_spec; intuition. Qed.
+    Lemma remove_2 : ~ E.eq x y -> In y cs -> In y (remove x cs).
+    Proof. intros; apply <- remove_spec; auto with relations. Qed.
+    Lemma remove_3 : In y (remove x cs) -> In y cs.
+    Proof. rewrite remove_spec; intuition. Qed.
+
+    Lemma singleton_1 : In y (singleton x) -> E.eq x y.
+    Proof. rewrite singleton_spec; auto with relations. Qed.
+    Lemma singleton_2 : E.eq x y -> In y (singleton x).
+    Proof. rewrite singleton_spec; auto with relations. Qed.
+
+    Lemma union_1 : In x (union cs1 cs2) -> In x cs1 \/ In x cs2.
+    Proof. rewrite union_spec; auto. Qed.
+    Lemma union_2 : In x cs1 -> In x (union cs1 cs2).
+    Proof. rewrite union_spec; auto. Qed.
+    Lemma union_3 : In x cs2 -> In x (union cs1 cs2).
+    Proof. rewrite union_spec; auto. Qed.
+
+    Lemma inter_1 : In x (inter cs1 cs2) -> In x cs1.
+    Proof. rewrite inter_spec; intuition. Qed.
+    Lemma inter_2 : In x (inter cs1 cs2) -> In x cs2.
+    Proof. rewrite inter_spec; intuition. Qed.
+    Lemma inter_3 : In x cs1 -> In x cs2 -> In x (inter cs1 cs2).
+    Proof. rewrite inter_spec; intuition. Qed.
+
+    Lemma diff_1 : In x (diff cs1 cs2) -> In x cs1.
+    Proof. rewrite diff_spec; intuition. Qed.
+    Lemma diff_2 : In x (diff cs1 cs2) -> ~ In x cs2.
+    Proof. rewrite diff_spec; intuition. Qed.
+    Lemma diff_3 : In x cs1 -> ~ In x cs2 -> In x (diff cs1 cs2).
+    Proof. rewrite diff_spec; auto. Qed.
+
+    Lemma disjoint_1 : Disjoint cs1 cs2 -> disjoint cs1 cs2 = true.
+    Proof. intros; apply <- disjoint_spec; auto. Qed.
+    Lemma disjoint_2 : disjoint cs1 cs2 = true -> Disjoint cs1 cs2.
+    Proof. intros; apply -> disjoint_spec; auto. Qed.
+
+  End ImplSpec.
+
+  Notation empty_1 := empty_spec (only parsing).
+  Notation universe_1 := universe_spec (only parsing).
+
+  Hint Resolve mem_1 equal_1 subset_1 empty_1 universe_1
+      is_empty_1 is_universe_1 add_1 add_2 remove_1
+      remove_2 singleton_2 union_1 union_2 union_3
+      inter_3 diff_3 disjoint_1 : set.
+
+  Hint Immediate In_1 mem_2 equal_2 subset_2 is_empty_2
+       is_universe_2 add_3 remove_3 singleton_1 inter_1
+       inter_2 diff_1 diff_2 disjoint_2
+    : set.
+
+  (** * Specifications written using equivalences :
+        this is now provided by the default interface. *)
+
+  Section IffSpec.
+    Variable cs cs1 cs2 : t.
+    Variable x y : elt.
+
+    Lemma In_eq_iff : E.eq x y -> (In x cs <-> In y cs).
+    Proof.
+      intros E; rewrite E; intuition.
+    Qed.
+
+    Lemma mem_iff : In x cs <-> mem x cs = true.
+    Proof. apply iff_sym, mem_spec. Qed.
+
+    Lemma not_mem_iff : ~In x cs <-> mem x cs = false.
+    Proof.
+      rewrite <-mem_spec; destruct (mem x cs); intuition.
+    Qed.
+
+    Lemma equal_iff : Equal cs1 cs2 <-> equal cs1 cs2 = true.
+    Proof. apply iff_sym, equal_spec. Qed.
+
+    Lemma subset_iff : Subset cs1 cs2 <-> subset cs1 cs2 = true.
+    Proof. apply iff_sym. apply subset_spec. Qed.
+
+    Lemma empty_iff : In x empty <-> False.
+    Proof. intuition; apply (empty_spec H). Qed.
+
+    Lemma universe_iff : In x universe <-> True.
+    Proof. intuition; apply (universe_spec H). Qed.
+
+    Lemma is_empty_iff : Empty cs <-> is_empty cs = true.
+    Proof. apply iff_sym, is_empty_spec. Qed.
+
+    Lemma is_universe_iff : Universe cs <-> is_universe cs = true.
+    Proof. apply iff_sym, is_universe_spec. Qed.
+
+    Lemma singleton_iff : In y (singleton x) <-> E.eq x y.
+    Proof. rewrite singleton_spec; intuition. Qed.
+
+    Lemma add_iff : In y (add x cs) <-> E.eq x y \/ In y cs.
+    Proof. rewrite add_spec; intuition. Qed.
+
+    Lemma add_neq_iff : ~ E.eq x y -> (In y (add x cs)  <-> In y cs).
+    Proof.
+      rewrite add_spec; intuition. elim H; auto with relations.
+    Qed.
+
+    Lemma remove_iff : In y (remove x cs) <-> In y cs /\ ~E.eq x y.
+    Proof. rewrite remove_spec; intuition. Qed.
+
+    Lemma remove_neq_iff :
+      ~ E.eq x y -> (In y (remove x cs) <-> In y cs).
+    Proof. rewrite remove_spec; intuition. Qed.
+
+    Lemma disjoint_iff : Disjoint cs1 cs2 <-> disjoint cs1 cs2 = true.
+    Proof. apply iff_sym. apply disjoint_spec. Qed.
+
+  End IffSpec.
+
+  Notation union_iff := union_spec (only parsing).
+  Notation inter_iff := inter_spec (only parsing).
+  Notation diff_iff := diff_spec (only parsing).
+
+  (** Useful tactic for simplifying expressions like
+      [In y (add x (union s s'))] *)
+
+  Ltac set_iff :=
+   repeat (progress (
+    rewrite add_iff || rewrite remove_iff || rewrite singleton_iff
+    || rewrite union_iff || rewrite inter_iff || rewrite diff_iff
+    || rewrite empty_iff || rewrite universe_iff)).
+
+  (**  * Specifications written using boolean predicates *)
+
+  Section BoolSpec.
+    Variable cs cs1 cs2 : t.
+    Variable x y : elt.
+
+    Lemma mem_b : E.eq x y -> mem x cs = mem y cs.
+    Proof.
+    intros.
+    generalize (mem_iff cs x) (mem_iff cs y)(In_eq_iff cs H).
+    destruct (mem x cs); destruct (mem y cs); intuition.
+    Qed.
+
+    Lemma empty_b : mem y empty = false.
+    Proof.
+    generalize (empty_iff y)(mem_iff empty y).
+    destruct (mem y empty); intuition.
+    Qed.
+
+    Lemma universe_b : mem y universe = true.
+    Proof.
+    generalize (universe_iff y)(mem_iff universe y).
+    destruct (mem y universe); intuition.
+    Qed.
+
+    Lemma add_b : mem y (add x cs) = eqb x y || mem y cs.
+    Proof.
+    generalize (mem_iff (add x cs) y)(mem_iff cs y)(add_iff cs x y);
+      unfold eqb.
+    destruct (eq_dec x y); destruct (mem y cs);
+      destruct (mem y (add x cs)); intuition.
+    Qed.
+
+    Lemma add_neq_b : ~ E.eq x y -> mem y (add x cs) = mem y cs.
+    Proof.
+    intros;
+      generalize (mem_iff (add x cs) y)
+        (mem_iff cs y) (add_neq_iff cs H).
+    destruct (mem y cs); destruct (mem y (add x cs)); intuition.
+    Qed.
+
+    Lemma remove_b : mem y (remove x cs) = mem y cs && negb (eqb x y).
+    Proof.
+    generalize (mem_iff (remove x cs) y)
+      (mem_iff cs y)(remove_iff cs x y);
+      unfold eqb.
+    destruct (eq_dec x y); destruct (mem y cs);
+      destruct (mem y (remove x cs)); simpl; intuition.
+    Qed.
+
+    Lemma remove_neq_b : ~ E.eq x y -> mem y (remove x cs) = mem y cs.
+    Proof.
+    intros; generalize (mem_iff (remove x cs) y)
+      (mem_iff cs y)(remove_neq_iff cs H).
+    destruct (mem y cs); destruct (mem y (remove x cs)); intuition.
+    Qed.
+
+    Lemma singleton_b : mem y (singleton x) = eqb x y.
+    Proof.
+    generalize (mem_iff (singleton x) y)(singleton_iff x y);
+      unfold eqb.
+    destruct (eq_dec x y); destruct (mem y (singleton x)); intuition.
+    Qed.
+
+    Lemma union_b : mem x (union cs1 cs2) = mem x cs1 || mem x cs2.
+    Proof.
+    generalize (mem_iff (union cs1 cs2) x)
+      (mem_iff cs1 x)(mem_iff cs2 x)(union_iff cs1 cs2 x).
+    destruct (mem x cs1); destruct (mem x cs2);
+      destruct (mem x (union cs1 cs2)); intuition.
+    Qed.
+
+    Lemma inter_b : mem x (inter cs1 cs2) = mem x cs1 && mem x cs2.
+    Proof.
+    generalize (mem_iff (inter cs1 cs2) x)
+      (mem_iff cs1 x)(mem_iff cs2 x)(inter_iff cs1 cs2 x).
+    destruct (mem x cs1); destruct (mem x cs2);
+      destruct (mem x (inter cs1 cs2)); intuition.
+    Qed.
+
+    Lemma diff_b :
+      mem x (diff cs1 cs2) = mem x cs1 && negb (mem x cs2).
+    Proof.
+    generalize (mem_iff (diff cs1 cs2) x)
+      (mem_iff cs1 x)(mem_iff cs2 x)(diff_iff cs1 cs2 x).
+    destruct (mem x cs1); destruct (mem x cs2);
+      destruct (mem x (diff cs1 cs2)); simpl; intuition.
+    Qed.
+
+  End BoolSpec.
+
+  (** * Declarations of morphisms with respects to [E.eq] and
+        [Equal] *)
+
+  Instance In_m : Proper (E.eq==>Equal==>iff) In.
+  Proof.
+  unfold Equal; intros x y H s s' H0.
+  rewrite (In_eq_iff s H); auto.
+  Qed.
+
+  Instance Empty_m : Proper (Equal==>iff) Empty.
+  Proof.
+  repeat red; unfold Empty; intros s s' E.
+  setoid_rewrite E; auto.
+  Qed.
+
+  Instance Universe_m : Proper (Equal==>iff) Universe.
+  Proof.
+  repeat red; unfold Universe; intros s s' E.
+  setoid_rewrite E; auto.
+  Qed.
+
+  Instance is_empty_m : Proper (Equal==>Logic.eq) is_empty.
+  Proof.
+  intros s s' H.
+  generalize (is_empty_iff s). rewrite H at 1. rewrite is_empty_iff.
+  destruct (is_empty s); destruct (is_empty s'); intuition.
+  Qed.
+
+  Instance is_universe_m : Proper (Equal==>Logic.eq) is_universe.
+  Proof.
+  intros s s' H.
+  generalize (is_universe_iff s).
+  rewrite H at 1. rewrite is_universe_iff.
+  destruct (is_universe s); destruct (is_universe s'); intuition.
+  Qed.
+
+  Instance mem_m : Proper (E.eq==>Equal==>Logic.eq) mem.
+  Proof.
+  intros x x' Hx s s' Hs.
+  generalize (mem_iff s x). rewrite Hs, Hx at 1; rewrite mem_iff.
+  destruct (mem x s), (mem x' s'); intuition.
+  Qed.
+
+  Instance singleton_m : Proper (E.eq==>Equal) singleton.
+  Proof.
+  intros x y H a. rewrite !singleton_iff, H; intuition.
+  Qed.
+
+  Instance add_m : Proper (E.eq==>Equal==>Equal) add.
+  Proof.
+  intros x x' Hx s s' Hs a. rewrite !add_iff, Hx, Hs; intuition.
+  Qed.
+
+  Instance remove_m : Proper (E.eq==>Equal==>Equal) remove.
+  Proof.
+  intros x x' Hx s s' Hs a. rewrite !remove_iff, Hx, Hs; intuition.
+  Qed.
+
+  Instance union_m : Proper (Equal==>Equal==>Equal) union.
+  Proof.
+  intros s1 s1' Hs1 s2 s2' Hs2 a.
+  rewrite !union_iff, Hs1, Hs2; intuition.
+  Qed.
+
+  Instance inter_m : Proper (Equal==>Equal==>Equal) inter.
+  Proof.
+  intros s1 s1' Hs1 s2 s2' Hs2 a.
+  rewrite !inter_iff, Hs1, Hs2; intuition.
+  Qed.
+
+  Instance diff_m : Proper (Equal==>Equal==>Equal) diff.
+  Proof.
+  intros s1 s1' Hs1 s2 s2' Hs2 a.
+  rewrite !diff_iff, Hs1, Hs2; intuition.
+  Qed.
+
+  Instance Subset_m : Proper (Equal==>Equal==>iff) Subset.
+  Proof.
+  unfold Equal, Subset; firstorder.
+  Qed.
+
+  Instance subset_m : Proper (Equal==>Equal==>Logic.eq) subset.
+  Proof.
+  intros s1 s1' Hs1 s2 s2' Hs2.
+  generalize (subset_iff s1 s2).
+  rewrite Hs1, Hs2 at 1. rewrite subset_iff.
+  destruct (subset s1 s2); destruct (subset s1' s2'); intuition.
+  Qed.
+
+  Instance equal_m : Proper (Equal==>Equal==>Logic.eq) equal.
+  Proof.
+  intros s1 s1' Hs1 s2 s2' Hs2.
+  generalize (equal_iff s1 s2).
+  rewrite Hs1,Hs2 at 1. rewrite equal_iff.
+  destruct (equal s1 s2); destruct (equal s1' s2'); intuition.
+  Qed.
+
+  Instance Disjoint_m : Proper (Equal==>Equal==>iff) Disjoint.
+  Proof.
+  unfold Equal, Disjoint; firstorder.
+  Qed.
+
+  Instance disjoint_m : Proper (Equal==>Equal==>Logic.eq) disjoint.
+  Proof.
+  intros s1 s1' Hs1 s2 s2' Hs2.
+  generalize (disjoint_iff s1 s2).
+  rewrite Hs1, Hs2 at 1. rewrite disjoint_iff.
+  destruct (disjoint s1 s2); destruct (disjoint s1' s2'); intuition.
+  Qed.
+
+  Instance SubsetSetoid : PreOrder Subset.
+  Proof. firstorder. Qed.
+
+  Definition Subset_refl := @PreOrder_Reflexive _ _ SubsetSetoid.
+  Definition Subset_trans := @PreOrder_Transitive _ _ SubsetSetoid.
+
+  Instance In_s_m :
+    Morphisms.Proper (E.eq ==> Subset ++> impl) In | 1.
+  Proof.
+    simpl_relation. fold (In y y0). eauto with set.
+  Qed.
+
+  Instance Empty_s_m : Proper (Subset-->impl) Empty.
+  Proof. firstorder. Qed.
+
+  Instance Universe_s_m : Proper (Subset-->impl) Empty.
+  Proof. firstorder. Qed.
+
+  Instance add_s_m : Proper (E.eq==>Subset++>Subset) add.
+  Proof.
+  intros x x' Hx s s' Hs a. rewrite !add_iff, Hx; intuition.
+  Qed.
+
+  Instance remove_s_m : Proper (E.eq==>Subset++>Subset) remove.
+  Proof.
+  intros x x' Hx s s' Hs a. rewrite !remove_iff, Hx; intuition.
+  Qed.
+
+  Instance union_s_m : Proper (Subset++>Subset++>Subset) union.
+  Proof.
+  intros s1 s1' Hs1 s2 s2' Hs2 a.
+  rewrite !union_iff, Hs1, Hs2; intuition.
+  Qed.
+
+  Instance inter_s_m : Proper (Subset++>Subset++>Subset) inter.
+  Proof.
+  intros s1 s1' Hs1 s2 s2' Hs2 a.
+  rewrite !inter_iff, Hs1, Hs2; intuition.
+  Qed.
+
+  Instance diff_s_m : Proper (Subset++>Subset-->Subset) diff.
+  Proof.
+  intros s1 s1' Hs1 s2 s2' Hs2 a.
+  rewrite !diff_iff, Hs1, Hs2; intuition.
+  Qed.
+
+End CSetFacts.
+
+(**************************************************************)
+(* CSetDecide                                                 *)
+(**************************************************************)
+
+Require Import Decidable Setoid DecidableTypeEx.
+
+(** * Facts and Tactics for Propositional Logic
+      These lemmas and tactics are in a module so that they do
+      not affect the namespace if you import the enclosing
+      module [Decide]. *)
+Module CSetLogicalFacts.
+
+  Export Decidable.
+  Export Setoid.
+
+  (** ** Lemmas and Tactics About Decidable Propositions *)
+
+  (** ** Propositional Equivalences Involving Negation
+        These are all written with the unfolded form of
+        negation, since I am not sure if setoid rewriting will
+        always perform conversion. *)
+
+  (** ** Tactics for Negations *)
+
+  Tactic Notation "fold" "any" "not" :=
+    repeat (
+      match goal with
+      | H: context [?P -> False] |- _ =>
+        fold (~ P) in H
+      | |- context [?P -> False] =>
+        fold (~ P)
+      end).
+
+  (** [push not using db] will pushes all negations to the
+      leaves of propositions in the goal, using the lemmas in
+      [db] to assist in checking the decidability of the
+      propositions involved.  If [using db] is omitted, then
+      [core] will be used.  Additional versions are provided
+      to manipulate the hypotheses or the hypotheses and goal
+      together. *)
+
+  Ltac or_not_l_iff P Q tac :=
+    (rewrite (or_not_l_iff_1 P Q) by tac) ||
+    (rewrite (or_not_l_iff_2 P Q) by tac).
+
+  Ltac or_not_r_iff P Q tac :=
+    (rewrite (or_not_r_iff_1 P Q) by tac) ||
+    (rewrite (or_not_r_iff_2 P Q) by tac).
+
+  Ltac or_not_l_iff_in P Q H tac :=
+    (rewrite (or_not_l_iff_1 P Q) in H by tac) ||
+    (rewrite (or_not_l_iff_2 P Q) in H by tac).
+
+  Ltac or_not_r_iff_in P Q H tac :=
+    (rewrite (or_not_r_iff_1 P Q) in H by tac) ||
+    (rewrite (or_not_r_iff_2 P Q) in H by tac).
+
+  Tactic Notation "push" "not" "using" ident(db) :=
+    let dec := solve_decidable using db in
+    unfold not, iff;
+    repeat (
+      match goal with
+      | |- context [True -> False] => rewrite not_true_iff
+      | |- context [False -> False] => rewrite not_false_iff
+      | |- context [(?P -> False) -> False] =>
+        rewrite (not_not_iff P) by dec
+      | |- context [(?P -> False) -> (?Q -> False)] =>
+          rewrite (contrapositive P Q) by dec
+      | |- context [(?P -> False) \/ ?Q] => or_not_l_iff P Q dec
+      | |- context [?P \/ (?Q -> False)] => or_not_r_iff P Q dec
+      | |- context [(?P -> False) -> ?Q] =>
+        rewrite (imp_not_l P Q) by dec
+      | |- context [?P \/ ?Q -> False] => rewrite (not_or_iff P Q)
+      | |- context [?P /\ ?Q -> False] => rewrite (not_and_iff P Q)
+      | |- context [(?P -> ?Q) -> False] =>
+        rewrite (not_imp_iff P Q) by dec
+      end);
+    fold any not.
+
+  Tactic Notation "push" "not" :=
+    push not using core.
+
+  Tactic Notation
+    "push" "not" "in" "*" "|-" "using" ident(db) :=
+    let dec := solve_decidable using db in
+    unfold not, iff in * |-;
+    repeat (
+      match goal with
+      | H: context [True -> False] |- _ =>
+        rewrite not_true_iff in H
+      | H: context [False -> False] |- _ =>
+        rewrite not_false_iff in H
+      | H: context [(?P -> False) -> False] |- _ =>
+        rewrite (not_not_iff P) in H by dec
+      | H: context [(?P -> False) -> (?Q -> False)] |- _ =>
+        rewrite (contrapositive P Q) in H by dec
+      | H: context [(?P -> False) \/ ?Q] |- _ =>
+        or_not_l_iff_in P Q H dec
+      | H: context [?P \/ (?Q -> False)] |- _ =>
+        or_not_r_iff_in P Q H dec
+      | H: context [(?P -> False) -> ?Q] |- _ =>
+        rewrite (imp_not_l P Q) in H by dec
+      | H: context [?P \/ ?Q -> False] |- _ =>
+        rewrite (not_or_iff P Q) in H
+      | H: context [?P /\ ?Q -> False] |- _ =>
+        rewrite (not_and_iff P Q) in H
+      | H: context [(?P -> ?Q) -> False] |- _ =>
+        rewrite (not_imp_iff P Q) in H by dec
+      end);
+    fold any not.
+
+  Tactic Notation "push" "not" "in" "*" "|-"  :=
+    push not in * |- using core.
+
+  Tactic Notation "push" "not" "in" "*" "using" ident(db) :=
+    push not using db; push not in * |- using db.
+  Tactic Notation "push" "not" "in" "*" :=
+    push not in * using core.
+
+  (** [pull not using db] will pull as many negations as
+      possible toward the top of the propositions in the goal,
+      using the lemmas in [db] to assist in checking the
+      decidability of the propositions involved.  If [using
+      db] is omitted, then [core] will be used.  Additional
+      versions are provided to manipulate the hypotheses or
+      the hypotheses and goal together. *)
+
+  Tactic Notation "pull" "not" "using" ident(db) :=
+    let dec := solve_decidable using db in
+    unfold not, iff;
+    repeat (
+      match goal with
+      | |- context [True -> False] => rewrite not_true_iff
+      | |- context [False -> False] => rewrite not_false_iff
+      | |- context [(?P -> False) -> False] =>
+        rewrite (not_not_iff P) by dec
+      | |- context [(?P -> False) -> (?Q -> False)] =>
+        rewrite (contrapositive P Q) by dec
+      | |- context [(?P -> False) \/ ?Q] => or_not_l_iff P Q dec
+      | |- context [?P \/ (?Q -> False)] => or_not_r_iff P Q dec
+      | |- context [(?P -> False) -> ?Q] =>
+        rewrite (imp_not_l P Q) by dec
+      | |- context [(?P -> False) /\ (?Q -> False)] =>
+        rewrite <- (not_or_iff P Q)
+      | |- context [?P -> ?Q -> False] =>
+        rewrite <- (not_and_iff P Q)
+      | |- context [?P /\ (?Q -> False)] =>
+        rewrite <- (not_imp_iff P Q) by dec
+      | |- context [(?Q -> False) /\ ?P] =>
+        rewrite <- (not_imp_rev_iff P Q) by dec
+      end);
+    fold any not.
+
+  Tactic Notation "pull" "not" :=
+    pull not using core.
+
+  Tactic Notation
+    "pull" "not" "in" "*" "|-" "using" ident(db) :=
+    let dec := solve_decidable using db in
+    unfold not, iff in * |-;
+    repeat (
+      match goal with
+      | H: context [True -> False] |- _ =>
+        rewrite not_true_iff in H
+      | H: context [False -> False] |- _ =>
+        rewrite not_false_iff in H
+      | H: context [(?P -> False) -> False] |- _ =>
+        rewrite (not_not_iff P) in H by dec
+      | H: context [(?P -> False) -> (?Q -> False)] |- _ =>
+        rewrite (contrapositive P Q) in H by dec
+      | H: context [(?P -> False) \/ ?Q] |- _ =>
+        or_not_l_iff_in P Q H dec
+      | H: context [?P \/ (?Q -> False)] |- _ =>
+        or_not_r_iff_in P Q H dec
+      | H: context [(?P -> False) -> ?Q] |- _ =>
+        rewrite (imp_not_l P Q) in H by dec
+      | H: context [(?P -> False) /\ (?Q -> False)] |- _ =>
+        rewrite <- (not_or_iff P Q) in H
+      | H: context [?P -> ?Q -> False] |- _ =>
+        rewrite <- (not_and_iff P Q) in H
+      | H: context [?P /\ (?Q -> False)] |- _ =>
+        rewrite <- (not_imp_iff P Q) in H by dec
+      | H: context [(?Q -> False) /\ ?P] |- _ =>
+        rewrite <- (not_imp_rev_iff P Q) in H by dec
+      end);
+    fold any not.
+
+  Tactic Notation "pull" "not" "in" "*" "|-"  :=
+    pull not in * |- using core.
+
+  Tactic Notation "pull" "not" "in" "*" "using" ident(db) :=
+    pull not using db; pull not in * |- using db.
+  Tactic Notation "pull" "not" "in" "*" :=
+    pull not in * using core.
+
+End CSetLogicalFacts.
+
+Import CSetLogicalFacts.
+
+Module CSetDecideAuxiliary.
+
+  (** ** Generic Tactics
+      We begin by defining a few generic, useful tactics. *)
+
+  Ltac no_logical_interdep :=
+    match goal with
+      | H : ?P |- _ =>
+        match type of P with
+          | Prop =>
+            match goal with
+              H' : context [ H ] |- _ =>
+              clear dependent H' end
+          | _ => fail
+        end; no_logical_interdep
+      | _ => idtac
+    end.
+
+  Ltac abstract_term t :=
+    tryif (is_var t) then fail "no need to abstract a variable"
+    else (let x := fresh "x" in set (x := t) in *; try clearbody x).
+
+  Ltac abstract_elements :=
+    repeat
+      (match goal with
+         | |- context [ singleton ?t ] => abstract_term t
+         | _ : context [ singleton ?t ] |- _ => abstract_term t
+         | |- context [ cosingleton ?t ] => abstract_term t
+         | _ : context [ cosingleton ?t ] |- _ => abstract_term t
+         | |- context [ add ?t _ ] => abstract_term t
+         | _ : context [ add ?t _ ] |- _ => abstract_term t
+         | |- context [ remove ?t _ ] => abstract_term t
+         | _ : context [ remove ?t _ ] |- _ => abstract_term t
+         | |- context [ In ?t _ ] => abstract_term t
+         | _ : context [ In ?t _ ] |- _ => abstract_term t
+       end).
+
+  (** [prop P holds by t] succeeds (but does not modify the
+      goal or context) if the proposition [P] can be proved by
+      [t] in the current context.  Otherwise, the tactic
+      fails. *)
+  Tactic Notation "prop" constr(P) "holds" "by" tactic(t) :=
+    let H := fresh in
+    assert P as H by t;
+    clear H.
+
+  (** This tactic acts just like [assert ... by ...] but will
+      fail if the context already contains the proposition. *)
+  Tactic Notation "assert" "new" constr(e) "by" tactic(t) :=
+    match goal with
+    | H: e |- _ => fail 1
+    | _ => assert e by t
+    end.
+
+  (** [subst++] is similar to [subst] except that
+      - it never fails (as [subst] does on recursive
+        equations),
+      - it substitutes locally defined variable for their
+        definitions,
+      - it performs beta reductions everywhere, which may
+        arise after substituting a locally defined function
+        for its definition.
+      *)
+  Tactic Notation "subst" "++" :=
+    repeat (
+      match goal with
+      | x : _ |- _ => subst x
+      end);
+    cbv zeta beta in *.
+
+  (** [decompose records] calls [decompose record H] on every
+      relevant hypothesis [H]. *)
+  Tactic Notation "decompose" "records" :=
+    repeat (
+      match goal with
+      | H: _ |- _ => progress (decompose record H); clear H
+      end).
+
+  (** ** Discarding Irrelevant Hypotheses
+      We will want to clear the context of any
+      non-MSet-related hypotheses in order to increase the
+      speed of the tactic.  To do this, we will need to be
+      able to decide which are relevant.  We do this by making
+      a simple inductive definition classifying the
+      propositions of interest. *)
+
+  Inductive MSet_elt_Prop : Prop -> Prop :=
+  | eq_Prop : forall (S : Type) (x y : S),
+      MSet_elt_Prop (x = y)
+  | eq_elt_prop : forall x y,
+      MSet_elt_Prop (E.eq x y)
+  | In_elt_prop : forall x s,
+      MSet_elt_Prop (In x s)
+  | True_elt_prop :
+      MSet_elt_Prop True
+  | False_elt_prop :
+      MSet_elt_Prop False
+  | conj_elt_prop : forall P Q,
+      MSet_elt_Prop P ->
+      MSet_elt_Prop Q ->
+      MSet_elt_Prop (P /\ Q)
+  | disj_elt_prop : forall P Q,
+      MSet_elt_Prop P ->
+      MSet_elt_Prop Q ->
+      MSet_elt_Prop (P \/ Q)
+  | impl_elt_prop : forall P Q,
+      MSet_elt_Prop P ->
+      MSet_elt_Prop Q ->
+      MSet_elt_Prop (P -> Q)
+  | not_elt_prop : forall P,
+      MSet_elt_Prop P ->
+      MSet_elt_Prop (~ P).
+
+  Inductive MSet_Prop : Prop -> Prop :=
+  | elt_MSet_Prop : forall P,
+      MSet_elt_Prop P ->
+      MSet_Prop P
+  | Empty_MSet_Prop : forall s,
+      MSet_Prop (Empty s)
+  | Universe_MSet_Prop : forall s,
+      MSet_Prop (Universe s)
+  | Subset_MSet_Prop : forall s1 s2,
+      MSet_Prop (Subset s1 s2)
+  | Equal_MSet_Prop : forall s1 s2,
+      MSet_Prop (Equal s1 s2)
+  | Disjoint_MSet_Prop : forall s1 s2,
+      MSet_Prop (Disjoint s1 s2).
+
+  (** Here is the tactic that will throw away hypotheses that
+      are not useful (for the intended scope of the [fsetdec]
+      tactic). *)
+  Hint Constructors MSet_elt_Prop MSet_Prop : MSet_Prop.
+  Ltac discard_nonMSet :=
+    repeat (
+      match goal with
+      | H : context [ @Logic.eq ?T ?x ?y ] |- _ =>
+        tryif (change T with E.t in H) then fail
+        else tryif (change T with t in H) then fail
+        else clear H
+      | H : ?P |- _ =>
+        tryif prop (MSet_Prop P) holds by
+          (auto 100 with MSet_Prop)
+        then fail
+        else clear H
+      end).
+
+  (** ** Turning Set Operators into Propositional Connectives
+      The lemmas from [MSetFacts] will be used to break down
+      set operations into propositional formulas built over
+      the predicates [In] and [E.eq] applied
+      only to variables.  We are going to use them with
+      [autorewrite].
+      *)
+
+  Hint Rewrite
+    CSetFacts.empty_iff CSetFacts.universe_iff
+    CSetFacts.singleton_iff CSetFacts.add_iff
+    CSetFacts.remove_iff CSetFacts.union_iff CSetFacts.inter_iff
+    CSetFacts.diff_iff
+  : set_simpl.
+
+  Lemma eq_refl_iff (x : elt) : x = x <-> True.
+  Proof.
+   now split.
+  Qed.
+
+  Hint Rewrite eq_refl_iff : set_eq_simpl.
+
+  (** ** Decidability of MSet Propositions *)
+
+  (** [In] is decidable. *)
+  Lemma dec_In : forall x s,
+    decidable (In x s).
+  Proof.
+    red; intros; generalize (CSetFacts.mem_iff s x);
+      case (mem x s); intuition.
+  Qed.
+
+  (** element equality is decidable. *)
+  Lemma dec_eq : forall (x y : elt),
+    decidable (x = y).
+  Proof.
+    red; intros x y; destruct (E.eq_dec x y); auto.
+  Qed.
+
+  (** The hint database [MSet_decidability] will be given to
+      the [push_neg] tactic from the module [Negation]. *)
+  Hint Resolve dec_In dec_eq : MSet_decidability.
+
+  (** ** Normalizing Propositions About Equality
+      We have to deal with the fact that [E.eq] may be
+      convertible with Coq's equality.  Thus, we will find the
+      following tactics useful to replace one form with the
+      other everywhere. *)
+
+  (** The next tactic, [Logic_eq_to_E_eq], mentions the term
+      [E.t]; thus, we must ensure that [E.t] is used in favor
+      of any other convertible but syntactically distinct
+      term. *)
+  Ltac change_to_E_t :=
+    repeat (
+      match goal with
+      | H : ?T |- _ =>
+        progress (change T with E.t in H);
+        repeat (
+          match goal with
+          | J : _ |- _ => progress (change T with E.t in J)
+          | |- _ => progress (change T with E.t)
+          end )
+      | H : forall x : ?T, _ |- _ =>
+        progress (change T with E.t in H);
+        repeat (
+          match goal with
+          | J : _ |- _ => progress (change T with E.t in J)
+          | |- _ => progress (change T with E.t)
+          end )
+     end).
+
+  (** These two tactics take us from Coq's built-in equality
+      to [E.eq] (and vice versa) when possible. *)
+
+  Ltac Logic_eq_to_E_eq :=
+    repeat (
+      match goal with
+      | H: _ |- _ =>
+        progress (change (@Logic.eq E.t) with E.eq in H)
+      | |- _ =>
+        progress (change (@Logic.eq E.t) with E.eq)
+      end).
+
+  Ltac E_eq_to_Logic_eq :=
+    repeat (
+      match goal with
+      | H: _ |- _ =>
+        progress (change E.eq with (@Logic.eq E.t) in H)
+      | |- _ =>
+        progress (change E.eq with (@Logic.eq E.t))
+      end).
+
+  (** This tactic works like the built-in tactic [subst], but
+      at the level of set element equality (which may not be
+      the convertible with Coq's equality). *)
+  Ltac substMSet :=
+    repeat (
+      match goal with
+      | H: E.eq ?x ?x |- _ => clear H
+      | H: E.eq ?x ?y |- _ => rewrite H in *; clear H
+      end);
+    autorewrite with set_eq_simpl in *.
+
+  (** ** Considering Decidability of Base Propositions
+      This tactic adds assertions about the decidability of
+      [E.eq] and [In] to the context.  This is necessary for
+      the completeness of the [fsetdec] tactic.  However, in
+      order to minimize the cost of proof search, we should be
+      careful to not add more than we need.  Once negations
+      have been pushed to the leaves of the propositions, we
+      only need to worry about decidability for those base
+      propositions that appear in a negated form. *)
+  Ltac assert_decidability :=
+    (** We actually don't want these rules to fire if the
+        syntactic context in the patterns below is trivially
+        empty, but we'll just do some clean-up at the
+        afterward.  *)
+    repeat (
+      match goal with
+      | H: context [~ E.eq ?x ?y] |- _ =>
+        assert new (E.eq x y \/ ~ E.eq x y) by (apply dec_eq)
+      | H: context [~ In ?x ?s] |- _ =>
+        assert new (In x s \/ ~ In x s) by (apply dec_In)
+      | |- context [~ E.eq ?x ?y] =>
+        assert new (E.eq x y \/ ~ E.eq x y) by (apply dec_eq)
+      | |- context [~ In ?x ?s] =>
+        assert new (In x s \/ ~ In x s) by (apply dec_In)
+      end);
+    (** Now we eliminate the useless facts we added (because
+        they would likely be very harmful to performance). *)
+    repeat (
+      match goal with
+      | _: ~ ?P, H : ?P \/ ~ ?P |- _ => clear H
+      end).
+
+  (** ** Handling [Empty], [Subset], and [Equal]
+      This tactic instantiates universally quantified
+      hypotheses (which arise from the unfolding of [Empty],
+      [Subset], and [Equal]) for each of the set element
+      expressions that is involved in some membership or
+      equality fact.  Then it throws away those hypotheses,
+      which should no longer be needed. *)
+  Ltac inst_MSet_hypotheses :=
+    repeat (
+      match goal with
+      | H : forall a : E.t, _,
+        _ : context [ In ?x _ ] |- _ =>
+        let P := type of (H x) in
+        assert new P by (exact (H x))
+      | H : forall a : E.t, _
+        |- context [ In ?x _ ] =>
+        let P := type of (H x) in
+        assert new P by (exact (H x))
+      | H : forall a : E.t, _,
+        _ : context [ E.eq ?x _ ] |- _ =>
+        let P := type of (H x) in
+        assert new P by (exact (H x))
+      | H : forall a : E.t, _
+        |- context [ E.eq ?x _ ] =>
+        let P := type of (H x) in
+        assert new P by (exact (H x))
+      | H : forall a : E.t, _,
+        _ : context [ E.eq _ ?x ] |- _ =>
+        let P := type of (H x) in
+        assert new P by (exact (H x))
+      | H : forall a : E.t, _
+        |- context [ E.eq _ ?x ] =>
+        let P := type of (H x) in
+        assert new P by (exact (H x))
+      end);
+    repeat (
+      match goal with
+      | H : forall a : E.t, _ |- _ =>
+        clear H
+      end).
+
+  (** ** The Core [fsetdec] Auxiliary Tactics *)
+
+  (** Here is the crux of the proof search.  Recursion through
+      [intuition]!  (This will terminate if I correctly
+      understand the behavior of [intuition].) *)
+  Ltac csetdec_rec := progress substMSet; intuition csetdec_rec.
+
+  (** If we add [unfold Empty, Subset, Equal in *; intros;] to
+      the beginning of this tactic, it will satisfy the same
+      specification as the [fsetdec] tactic; however, it will
+      be much slower than necessary without the pre-processing
+      done by the wrapper tactic [fsetdec]. *)
+  Ltac csetdec_body :=
+    autorewrite with set_eq_simpl in *;
+    inst_MSet_hypotheses;
+    autorewrite with set_simpl set_eq_simpl in *;
+    push not in * using MSet_decidability;
+    substMSet;
+    assert_decidability;
+    auto;
+    (intuition csetdec_rec) ||
+    fail 1
+      "because the goal is beyond the scope of this tactic".
+
+End CSetDecideAuxiliary.
+
+Import CSetDecideAuxiliary.
+
+(** * The [csetdec] Tactic
+    Here is the top-level tactic (the only one intended for
+    clients of this library).  It's specification is given at
+    the top of the file. *)
+Ltac csetdec :=
+  (** We first unfold any occurrences of [iff]. *)
+  unfold iff in *;
+  (** We fold occurrences of [not] because it is better for
+      [intros] to leave us with a goal of [~ P] than a goal of
+      [False]. *)
+  fold any not; intros;
+  (** We don't care about the value of elements : complex ones are
+      abstracted as new variables (avoiding potential dependencies,
+      see bug #2464) *)
+  abstract_elements;
+  (** We remove dependencies to logical hypothesis. This way,
+      later "clear" will work nicely (see bug #2136) *)
+  no_logical_interdep;
+  (** Now we decompose conjunctions, which will allow the
+      [discard_nonMSet] and [assert_decidability] tactics to
+      do a much better job. *)
+  decompose records;
+  discard_nonMSet;
+  (** We unfold these defined propositions on finite sets.  If
+      our goal was one of them, then have one more item to
+      introduce now. *)
+  unfold Empty, Universe, Subset, Disjoint, Equal in *; intros;
+  (** We now want to get rid of all uses of [=] in favor of
+      [E.eq].  However, the best way to eliminate a [=] is in
+      the context is with [subst], so we will try that first.
+      In fact, we may as well convert uses of [E.eq] into [=]
+      when possible before we do [subst] so that we can even
+      more mileage out of it.  Then we will convert all
+      remaining uses of [=] back to [E.eq] when possible.  We
+      use [change_to_E_t] to ensure that we have a canonical
+      name for set elements, so that [Logic_eq_to_E_eq] will
+      work properly.  *)
+  change_to_E_t; E_eq_to_Logic_eq; subst++; Logic_eq_to_E_eq;
+  (** The next optimization is to swap a negated goal with a
+      negated hypothesis when possible.  Any swap will improve
+      performance by eliminating the total number of
+      negations, but we will get the maximum benefit if we
+      swap the goal with a hypotheses mentioning the same set
+      element, so we try that first.  If we reach the fourth
+      branch below, we attempt any swap.  However, to maintain
+      completeness of this tactic, we can only perform such a
+      swap with a decidable proposition; hence, we first test
+      whether the hypothesis is an [MSet_elt_Prop], noting
+      that any [MSet_elt_Prop] is decidable. *)
+  pull not using MSet_decidability;
+  unfold not in *;
+  match goal with
+  | H: (In ?x ?r) -> False |- (In ?x ?s) -> False =>
+    contradict H; csetdec_body
+  | H: (In ?x ?r) -> False |- (E.eq ?x ?y) -> False =>
+    contradict H; csetdec_body
+  | H: (In ?x ?r) -> False |- (E.eq ?y ?x) -> False =>
+    contradict H; csetdec_body
+  | H: ?P -> False |- ?Q -> False =>
+    tryif prop (MSet_elt_Prop P) holds by
+      (auto 100 with MSet_Prop)
+    then (contradict H; csetdec_body)
+    else csetdec_body
+  | |- _ =>
+    csetdec_body
+  end.
+
+    
