Kinding.v
@@ -1,0 +1,625 @@
+(************************************************
+ *          Row Subtyping - Kinding             *
+ *                 Leo White                    *
+ ************************************************)
+
+Set Implicit Arguments.
+Require Import LibLN Definitions Infrastructure.
+
+(* *************************************************************** *)
+(** Uniqueness *)
+
+Lemma kinding_unique : forall E T K1 K2,
+    kinding E T K1 ->
+    kinding E T K2 ->
+    K1 = K2.
+Proof.
+  introv Hk1 Hk2.
+  gen K2.
+  induction Hk1; introv Hk2; inversion Hk2; subst; auto.
+  - lets Hke : (binds_func H0 H4).
+    inversion Hke; auto.
+  - lets Hke1 : (IHHk1_1 _ H3).
+    lets Hke2 : (IHHk1_2 _ H4).
+    inversion Hke1.
+    inversion Hke2.
+    reflexivity.
+Qed.
+
+Lemma kinding_unique_row : forall E T cs1 cs2,
+    kinding E T (knd_row cs1) ->
+    kinding E T (knd_row cs2) ->
+    cs1 = cs2.
+Proof.
+  introv H1 H2.
+  remember (kinding_unique H1 H2) as Heq.
+  inversion Heq.
+  easy.
+Qed.
+
+(* =============================================================== *)
+(** ** Automation for kinding *)
+
+Hint Resolve cons_non_empty_kind : kinding.
+
+Ltac unlessInList X Xs T :=
+  let b := inList X Xs in
+  match b with
+  | true => fail 1
+  | false => constr:T
+  end.
+
+Ltac find_kinding Ts :=
+  match goal with
+  | [ H : kinding _ (typ_constructor ?c ?T) _ |- _ ] =>
+    unlessInList (typ_constructor c T) Ts H
+  | [ H : kinding _ (typ_or ?T1 ?T2) _ |- _ ] =>
+    unlessInList (typ_or T1 T2) Ts H
+  | [ H : kinding _ (typ_variant ?T1 ?T2) _ |- _ ] =>
+    unlessInList (typ_variant T1 T2) Ts H
+  | [ H : kinding _ (typ_arrow ?T1 ?T2) _ |- _ ] =>
+    unlessInList (typ_arrow T1 T2) Ts H
+  | [ H : kinding _ (typ_meet ?T1 ?T2) _ |- _ ] =>
+    unlessInList (typ_meet T1 T2) Ts H
+  | [ H : kinding _ (typ_join ?T1 ?T2) _ |- _ ] =>
+    unlessInList (typ_join T1 T2) Ts H
+  | [ H : kinding _ (typ_top ?cs) _ |- _ ] =>
+    unlessInList (typ_top cs) Ts H
+  | [ H : kinding _ (typ_bot ?cs) _ |- _ ] =>
+    unlessInList (typ_bot cs) Ts H
+  end.
+
+Ltac kinding_type H :=
+  match type of H with
+  | kinding _ ?T _ => constr:T
+  end.
+
+Ltac invert_kinding_rec Ts :=
+  try
+    (let H := find_kinding Ts in
+     let T := kinding_type H in
+     inversion H;
+     invert_kinding_rec (T, Ts)).
+
+Ltac is_simple cs :=
+  match cs with
+  | cons_union _ _ => constr:false
+  | cons_inter _ _ => constr:false
+  | cons_universe => constr:false
+  | cons_diff _ _ => constr:false
+  | _ => constr:true
+  end.
+
+Ltac invert_knd_row_equal :=
+  repeat
+    match goal with
+    | H : knd_row ?cs = knd_row ?cs |- _ =>
+      clear H
+    | H : knd_row ?cs1 = knd_row ?cs2 |- _ =>
+      let var1 := is_simple cs1 in
+      match var1 with
+      | true =>
+        replace cs1 with cs2 in * by
+            (inversion H; reflexivity)
+      | false =>
+        let var2 := is_simple cs2 in
+        match var2 with
+        | true =>
+          replace cs2 with cs1 in * by
+              (inversion H; reflexivity)
+        | false =>
+          idtac
+        end
+      end
+    end.
+
+Ltac unique_kinding :=
+  repeat
+    match goal with
+    | H1 : kinding ?E ?T ?K,
+      H2 : kinding ?E ?T ?K |- _ =>
+      clear H1
+    | H1 : kinding ?E ?T (knd_row ?cs1),
+      H2 : kinding ?E ?T (knd_row ?cs2) |- _ =>
+      replace cs1 with cs2 in *
+        by (apply (kinding_unique_row H2 H1))
+    | H1 : kinding ?E ?T ?K1,
+      H2 : kinding ?E ?T ?K2 |- _ =>
+      replace K1 with K2 in *
+        by apply (kinding_unique H2 H1)
+    end.
+
+Ltac invert_kinding :=
+  invert_kinding_rec tt;
+  subst;
+  invert_knd_row_equal;
+  unique_kinding.
+
+(* *************************************************************** *)
+(** Weakening *)
+
+Hint Resolve binds_weaken : weaken.
+
+Lemma kinding_weakening : forall E F G T K,
+   kinding (E & G) T K -> 
+   environment (E & F & G) ->
+   kinding (E & F & G) T K.
+Proof.
+  introv Hk He.
+  inductions Hk; eauto with weaken.
+Qed.
+
+Hint Resolve kinding_weakening : weaken.
+
+Lemma kinding_weakening_l : forall E F T K,
+    kinding E T K ->
+    environment (E & F) ->
+    kinding (E & F) T K.
+Proof.
+  introv Hk He.
+  rewrite <- (concat_empty_r E) in Hk.
+  rewrite <- (concat_empty_r F) in *.
+  rewrite (concat_assoc E F empty) in *.
+  apply* kinding_weakening.
+Qed.
+
+Hint Resolve kinding_weakening_l : weaken.
+
+Lemma kinding_weakening_r : forall E F T K,
+    kinding E T K ->
+    environment (F & E) ->
+    kinding (F & E) T K.
+Proof.
+  introv Hk He.
+  rewrite <- (concat_empty_l E) in Hk.
+  rewrite <- (concat_empty_l F) in *.
+  apply* kinding_weakening.
+Qed.
+
+Hint Resolve kinding_weakening_r : weaken.
+
+Lemma kindings_weakening : forall E F G n Ts Ks,
+   kindings (E & G) n Ts Ks -> 
+   environment (E & F & G) ->
+   kindings (E & F & G) n Ts Ks.
+Proof.
+  introv Hk He.
+  gen_eq EG : (E & G).
+  induction Hk; intro; subst; auto.
+  - apply kindings_nil; auto.
+  - apply kindings_cons; auto with weaken.
+Qed.
+
+Hint Resolve kindings_weakening : weaken.
+
+Lemma kinding_body_weakening : forall E F G n Ks T,
+    kinding_body (E & G) n Ks T ->
+    length Ks = n ->
+    environment (E & F & G) ->
+    kinding_body (E & F & G) n Ks T.
+Proof.
+  introv Hk He.
+  destruct (kinding_body_regular Hk) as [_ [Hkd _]].
+  unfold kinding_body in *.
+  destruct Hk as [L Hk].
+  exists_fresh Xs Hf.
+  split; auto.
+  apply_ih_bind kinding_weakening.
+  - apply Hk; auto.
+  - apply environment_kinds with n; auto.
+    + rewrite! dom_concat.
+      auto.
+    + destruct Hkd; auto.
+Qed.
+
+Hint Resolve kinding_body_weakening : weaken.
+
+Lemma kinding_scheme_weakening : forall E F G M,
+    kinding_scheme (E & G) M ->
+    environment (E & F & G) ->
+    kinding_scheme (E & F & G) M.
+Proof.
+  unfold kinding_scheme.
+  introv Hk He.
+  apply* kinding_body_weakening.
+Qed.
+
+Hint Resolve kinding_scheme_weakening : weaken.
+
+Lemma kinding_scheme_weakening_l : forall E F M,
+    kinding_scheme E M ->
+    environment (E & F) ->
+    kinding_scheme (E & F) M.
+Proof.
+  introv Hk He.
+  rewrite <- (concat_empty_r E) in Hk.
+  rewrite <- (concat_empty_r F) in *.
+  rewrite (concat_assoc E F empty) in *.
+  apply* kinding_scheme_weakening.
+Qed.  
+
+Hint Resolve kinding_scheme_weakening_l : weaken.
+
+(* *************************************************************** *)
+(** Not affected by type bindings *)
+
+Lemma kinding_bind_typ : forall E F T K x S,
+    kinding (E & x ~: S & F) T K ->
+    kinding (E & F) T K.
+Proof.
+  introv Hk.
+  gen_eq Ex : (E & x ~: S & F).
+  induction Hk; intro; subst; eauto.
+  destruct (binds_middle_inv H0) as [|[[_[_ Heq]]|]]; iauto.
+  inversion Heq.
+Qed.
+
+Lemma kinding_bind_typ_l : forall E T K x S,
+    kinding (E & x ~: S) T K ->
+    kinding E T K.
+Proof.
+  introv Hk.
+  rewrite <- concat_empty_r with (E := E).
+  apply kinding_bind_typ with (x := x) (S := S).
+  rewrite concat_empty_r.
+  auto.
+Qed.
+
+Lemma kindings_bind_typ : forall E F n T K x S,
+    kindings (E & x ~: S & F) n T K ->
+    kindings (E & F) n T K.
+Proof.
+  introv Hk.
+  gen_eq G : (E & x ~: S & F).
+  induction Hk; intros; subst.
+  - apply* kindings_nil.
+  - apply* kindings_cons.
+    apply kinding_bind_typ with (x := x) (S := S).
+    auto.
+Qed.
+
+Lemma kinding_scheme_bind_typ : forall E F M x S,
+    kinding_scheme (E & x ~: S & F) M ->
+    kinding_scheme (E & F) M.
+Proof.
+  unfold kinding_scheme, kinding_body.
+  introv [L Hk].
+  exists_fresh Xs HFr.
+  destruct Hk with Xs as [Hkd Hks]; auto.
+  split; auto.
+  rewrite <- concat_assoc.
+  apply kinding_bind_typ with (x := x) (S := S).
+  rewrite concat_assoc.
+  auto.
+Qed.
+
+Hint Resolve kinding_bind_typ : bind_typ.
+Hint Resolve kinding_bind_typ_l : bind_typ.
+Hint Resolve kindings_bind_typ : bind_typ.
+Hint Resolve kinding_scheme_bind_typ : bind_typ.
+
+(* *************************************************************** *)
+(** Preserved by type substitution *)
+
+Lemma kinding_typ_subst : forall E F X T S K J,
+  kinding (E & X ~:: J & F) T K -> 
+  kinding E S J -> 
+  kinding (E & (environment_subst X S F)) (typ_subst X S T) K.
+Proof.
+  introv Hkt Hks.
+  gen_eq G : (E & X ~:: J & F).
+  induction Hkt; introv Heq; subst; simpl typ_subst; eauto.
+  - case_var.
+    + lets Hb : (binds_middle_eq_inv H0 (ok_from_environment H)).
+      inversion Hb; subst.
+      apply* kinding_weakening_l.
+    + { apply* kinding_var.
+        - apply binds_subst_inv_r.
+          eapply binds_subst.
+          + apply H0.
+          + auto. }
+Qed.
+
+Lemma kinding_typ_subst_l : forall E X T S K J,
+  kinding (E & X ~:: J) T K -> 
+  kinding E S J -> 
+  kinding E (typ_subst X S T) K.
+Proof.
+  introv Hk1 Hk2.
+  rewrite <- concat_empty_r with (E := E).
+  rewrite <- environment_subst_empty with (X := X) (T := S).
+  apply kinding_typ_subst with (J := J); auto.
+  rewrite concat_empty_r.
+  auto.
+Qed.
+
+Lemma kinding_typ_substs : forall E F Xs T Ss K Js n,
+  kinding (E & Xs ~::* Js & F) T K -> 
+  kindings E n Ss Js -> 
+  length Xs = n ->
+  length Js = n ->
+  length Ss = n ->
+  kinding (E & (environment_substs Xs Ss F)) (typ_substs Xs Ss T) K.
+Proof.
+  intros.
+  gen Ss Js T F n.
+  induction Xs; destruct Js; destruct Ss;
+    introv Hkt Hks; intros; subst; tryfalse; rew_kinds* in Hkt.
+  inversion Hks.
+  eapply IHXs; eauto.
+  eapply kinding_typ_subst.
+  - apply Hkt.
+  - apply* kinding_weakening_l.
+    eauto using environment_concat_inv_l.
+Qed.
+
+Lemma kinding_typ_substs_l : forall E Xs T Ss K Js n,
+  kinding (E & Xs ~::* Js) T K -> 
+  kindings E n Ss Js -> 
+  length Xs = n ->
+  length Js = n ->
+  length Ss = n ->
+  kinding E (typ_substs Xs Ss T) K.
+Proof.
+  introv Hk1 Hk2 Hlx Hlj Hls.
+  rewrite <- concat_empty_r with (E := E).
+  rewrite <- environment_substs_empty with (Xs := Xs) (Ts := Ss).
+  - apply kinding_typ_substs with (Js := Js) (n := n); auto.
+    rewrite concat_empty_r.
+    auto.
+  - subst*.
+Qed.
+
+Lemma kindings_typ_subst : forall n E F X Ts S Ks J,
+  kindings (E & X ~:: J & F) n Ts Ks -> 
+  kinding E S J -> 
+  kindings (E & (environment_subst X S F)) n
+           (List.map (typ_subst X S) Ts) Ks.
+Proof.
+  introv Hks Hk.
+  gen_eq G : (E & X ~:: J & F).
+  induction Hks; intro; subst; simpl.
+  - apply kindings_nil.
+    destruct* (environment_kind_middle_inv H).
+  - apply kindings_cons; auto.
+    apply kinding_typ_subst with J; auto.
+Qed.
+
+Lemma kinding_scheme_typ_subst : forall E F M X T K,
+    kinding_scheme (E & X ~:: K & F) M ->
+    kinding E T K ->
+    kinding_scheme (E & environment_subst X T F) (sch_subst X T M).
+Proof.
+  unfold kinding_scheme, kinding_body.
+  introv [L Hs] Ht.
+  exists_fresh Xs Hf.
+  unfold sch_arity in Hf.
+  lets Hlx : (fresh_length _ _ _ Hf).
+  lets Hf2 : Hf.
+  rewrite Hlx in Hf2.
+  apply fresh_length_arity_subst in Hf.
+  destruct Hs with Xs as [Hkd Hks]; auto.
+  split; auto.
+  rewrite <- concat_assoc.
+  rewrite* <- environment_subst_kinds.
+  fold (sch_open_vars (sch_subst X T M) Xs).
+  rewrite* <- sch_subst_open_vars.
+  unfold sch_open_vars.
+  apply kinding_typ_subst with (J := K); auto.
+  rewrite concat_assoc.
+  unfold sch_subst.
+  simpl.
+  apply Hs.
+  unfold sch_arity.
+  unfold sch_subst in Hf.
+  simpl in Hf.
+  auto.
+Qed.
+
+Hint Resolve kinding_typ_subst : typ_subst.
+Hint Resolve kinding_typ_subst_l : typ_subst.
+Hint Resolve kinding_typ_substs : typ_subst.
+Hint Resolve kinding_typ_substs_l : typ_subst.
+Hint Resolve kindings_typ_subst : typ_subst.
+
+Lemma kinding_sch_open : forall E M Ts,
+  kinding_scheme E M ->
+  kindings E (sch_arity M) Ts (sch_kinds M) ->
+  kinding E (sch_open M Ts) knd_type.
+Proof.
+  introv Hks Hkt.
+  destruct Hks as [L Hks].
+  pick_freshes (sch_arity M) Xs.
+  destruct Hks with Xs as [Hkd Hkk]; auto.
+  lets Hlx : (fresh_length _ _ _ Fr).
+  lets Hlk : (proj1 (proj32 (kindings_regular Hkt))).
+  rewrite* (@typ_substs_intro_sch M Xs Ts).
+  unfold sch_open_vars.
+  apply kinding_typ_substs_l
+    with (Js := sch_kinds M) (n := sch_arity M); auto.
+Qed.
+
+Hint Resolve kinding_sch_open : kinding.
+ 
+(* *************************************************************** *)
+(** Kinding of schemes with no parameters *)
+
+Lemma kinding_scheme_no_params : forall E T M,
+    kinding E T knd_type ->
+    M = Sch nil T ->
+    kinding_scheme E M.
+Proof.
+  introv Hk Heq.
+  subst.
+  exists_fresh Xs Hf.
+  simpl.
+  destruct (List.length_zero_iff_nil Xs) as [Hlz _].
+  rewrite (Hlz (eq_sym (fresh_length _ _ _ Hf))).
+  rewrite singles_nil.
+  rewrite map_empty.
+  rewrite concat_empty_r.
+  unfold typ_open_vars.
+  rewrite* <- (@typ_open_type T (typ_fvars nil)).
+Qed.
+
+(* *************************************************************** *)
+(** * Properties of well-kinded environments *)
+
+Lemma kinding_env_shorten : forall E G,
+    kinding_env (E & G) ->
+    kinding_env E.
+Proof.
+  introv Hk.
+  induction G using env_ind;
+    autorewrite with rew_env_concat in Hk; auto.
+  inversion Hk.
+  - destruct (empty_concat_inv H0) as [ He1 _ ].
+    destruct (empty_concat_inv He1) as [ He2 _ ].
+    rewrite* <- He2.
+  - destruct (eq_push_inv H) as [ _ [ _ He ] ].
+    subst*.
+  - destruct (eq_push_inv H) as [ _ [ _ He ] ].
+    subst*.
+Qed.
+
+Lemma kinding_env_kinds : forall E n Ks Xs,
+    kinding_env E ->
+    (fresh (dom E) n Xs) ->
+    kinds n Ks ->
+    kinding_env (E & Xs ~::* Ks).
+Proof.
+  introv Hk Hf Hlk.
+  lets Hlx : (eq_sym (fresh_length _ _ _ Hf)).
+  gen Ks n.
+  unfold kinds.
+  induction Xs; destruct Ks;
+    introv Hf [Hlk Hkd] Hlx; subst; tryfalse; rew_kinds*.
+  apply kinding_env_kind.
+  - apply IHXs with (length Ks); auto.
+    destruct* Hf.
+    inversion Hkd.
+    split; auto.
+  - inversion Hkd.
+    auto.
+  - eapply fresh_kinds; auto.
+Qed.
+
+Hint Resolve kinding_env_kinds : kinding.
+
+Lemma kinding_env_typ_push_inv : forall E x M,
+    kinding_env (E & x ~: M) ->
+    kinding_env E /\ x # E /\ kinding_scheme E M.
+Proof.
+  introv H.
+  inverts H as H1 H2 H3 H4.
+  - false (empty_push_inv H1).
+  - destruct (eq_push_inv H4) as [_ [Hv _]].
+    false Hv.
+  - destruct (eq_push_inv H4) as [Hx [Hv He]].
+    inversion Hv.
+    subst.
+    easy.
+Qed.
+
+Lemma kinding_env_kind_push_inv : forall E x K,
+    kinding_env (E & x ~:: K) ->
+    kinding_env E /\ x # E.
+Proof.
+  introv H.
+  inverts H as H1 H2 H3 H4.
+  - false (empty_push_inv H1).
+  - destruct (eq_push_inv H4) as [Hx [_ He]].
+    subst.
+    easy.
+  - destruct (eq_push_inv H4) as [_ [Hv _]].
+    false Hv.
+Qed.
+
+Lemma kinding_scheme_from_env : forall E x M,
+    kinding_env E ->
+    binds x (bind_typ M) E ->
+    kinding_scheme E M.
+Proof.
+  introv He Hb.
+  induction E using env_ind; rew_env_concat.
+  - false (binds_empty_inv Hb).
+  - destruct (binds_push_inv Hb); jauto_set.
+    + subst.
+      destruct (kinding_env_typ_push_inv He).
+      jauto_set.
+      auto with weaken.
+    + eauto using kinding_env_shorten with weaken.
+Qed.
+
+Hint Resolve kinding_scheme_from_env : kinding.
+
+Lemma kinding_env_well_scoped : forall E F X B,
+    kinding_env (E & X ~ B & F) ->
+    X \notin (env_fv E).
+Proof.
+  introv Hkef Hfv.
+  assert (kinding_env E) as Hke by eauto using kinding_env_shorten. 
+  lets Hd : (kinding_env_closed Hke Hfv).
+  assert (ok (E & X ~ B & F)) as Hok by auto.
+  apply ok_middle_inv in Hok.
+  iauto.
+Qed.
+
+(* *************************************************************** *)
+(** Not affected by type bindings *)
+
+Lemma kinding_env_bind_typ : forall E F x M,
+    kinding_env (E & x ~: M & F) ->
+    kinding_env (E & F).
+Proof.
+  introv Hk.
+  induction F using env_ind.
+  - rewrite concat_empty_r.
+    eauto using kinding_env_shorten.
+  - rewrite concat_assoc in *.
+    inversion Hk.
+    + apply empty_push_inv in H0.
+      tryfalse.
+    + destruct (eq_push_inv H) as [Ha [Hb Hc]].
+      subst.
+      apply kinding_env_kind; auto.
+    + destruct (eq_push_inv H) as [Ha [Hb Hc]].
+      subst; eauto using kinding_scheme_bind_typ.
+Qed.
+
+Hint Resolve kinding_env_bind_typ : bind_typ.
+
+(* *************************************************************** *)
+(** Preserved by type substitution *)
+
+Lemma kinding_env_typ_subst : forall E F X K T,
+  kinding_env (E & X ~:: K & F) -> 
+  kinding E T K -> 
+  kinding_env (E & (environment_subst X T F)).
+Proof.
+  introv He Hk.
+  induction F using env_ind.
+  - rewrite environment_subst_empty.
+    rewrite concat_empty_r.
+    eauto using kinding_env_shorten.
+  - rewrite environment_subst_push.
+    rewrite concat_assoc.
+    rewrite concat_assoc in He.
+    destruct v; simpl binding_subst.
+    + { destruct (kinding_env_kind_push_inv He).
+        apply kinding_env_kind; auto.
+        - lets Hee : (kinding_env_regular He).
+          apply kind_from_env with
+            (E := E & X ~:: K & F & x ~:: k)
+            (x := x); auto.
+        - rewrite dom_concat.
+          rewrite dom_environment_subst.
+          auto. }
+    + { destruct (kinding_env_typ_push_inv He) as [H1 [H2 H3]].
+        apply kinding_env_typ; auto.
+        - apply kinding_scheme_typ_subst with K; auto.
+        - rewrite dom_concat.
+          rewrite* dom_environment_subst. }
+Qed.
+
+Hint Resolve kinding_env_typ_subst: typ_subst.
