Subtyping.v
@@ -1,0 +1,908 @@
+(************************************************
+ *          Row Subtyping - Subtyping           *
+ *                 Leo White                    *
+ ************************************************)
+
+Set Implicit Arguments.
+Require Import LibLN Definitions Infrastructure Kinding.
+
+(* *************************************************************** *)
+(** * Properties of type equality *)
+
+(* *************************************************************** *)
+(** Transitivity *)
+
+Lemma type_equal_trans : forall E T1 T2 T3 K,
+    type_equal E T1 T2 K ->
+    type_equal E T2 T3 K ->
+    type_equal E T1 T3 K.
+Proof.
+  introv He.
+  induction He; eauto.
+Qed.
+
+(* *************************************************************** *)
+(** Well-kindedness *)
+
+Lemma type_equal_step_kinding : forall E T1 T2,
+    type_equal_step E T1 T2 ->
+    (forall K, kinding E T1 K -> kinding E T2 K)
+    /\ (forall K, kinding E T2 K -> kinding E T1 K).
+Proof.
+  introv Hs.
+  induction Hs;
+    split; intuition auto;
+      invert_kinding; eauto;
+        eauto with constrs.
+Qed.
+
+Lemma type_equal_kinding : forall E T1 T2 K,
+    type_equal E T1 T2 K ->
+    kinding E T1 K /\ kinding E T2 K.
+Proof.
+  introv He.
+  induction He; intuition auto.
+  - apply type_equal_step_kinding in H.
+    intuition auto.
+  - apply type_equal_step_kinding in H.
+    intuition auto.
+Qed.
+
+Hint Extern 1 (kinding ?E ?T ?K) =>
+  match goal with
+  | H: type_equal E T _ K |- _ =>
+      apply (proj1 (type_equal_kinding H))
+  | H: type_equal E _ T K |- _ =>
+      apply (proj2 (type_equal_kinding H))
+  end : kinding.
+
+(* *************************************************************** *)
+(** Symmetry *)
+
+Lemma type_equal_symm : forall E T1 T2 K,
+    type_equal E T1 T2 K ->
+    type_equal E T2 T1 K.
+Proof.
+  introv He.
+  induction He; auto.
+  - destruct (type_equal_step_kinding H).
+    destruct (type_equal_kinding He).
+    eapply type_equal_trans; eauto.
+  - destruct (type_equal_step_kinding H).
+    destruct (type_equal_kinding He).
+    eapply type_equal_trans; eauto.
+Qed.
+
+(* *************************************************************** *)
+(** Single steps *)
+
+Lemma type_equal_single_l : forall E T1 T2 K,
+    kinding E T2 K ->
+    type_equal_step E T1 T2 ->
+    type_equal E T1 T2 K.
+Proof.
+  introv Hk Hs.
+  eauto.
+Qed.
+
+Lemma type_equal_single_r : forall E T1 T2 K,
+    kinding E T1 K ->
+    type_equal_step E T1 T2 ->
+    type_equal E T2 T1 K.
+Proof.
+  introv Hk Hs.
+  eauto.
+Qed.
+
+(* *************************************************************** *)
+(** Congruence *)
+
+Lemma type_equal_constructor : forall E c T1 T1' K,
+    type_equal E T1 T1' knd_type ->
+    K = knd_row (cons_finite \{c}) ->
+    type_equal E (typ_constructor c T1) (typ_constructor c T1') K.
+Proof.
+  introv He Hkeq.
+  gen_eq K' : knd_type.
+  induction He; intros; subst; eauto with kinding.
+Qed.
+  
+Lemma type_equal_or : forall E T1 T1' T2 T2' cs1 cs2 K,
+      type_equal E T1 T1' (knd_row cs1) ->
+      type_equal E T2 T2' (knd_row cs2) ->
+      cons_disjoint cs1 cs2 ->
+      K = knd_row (cons_union cs1 cs2) ->
+      type_equal E (typ_or T1 T2) (typ_or T1' T2') K.
+Proof.
+  introv He1 He2 Hdis Hkeq.
+  apply type_equal_trans with (typ_or T1' T2).
+  - gen_eq K' : (knd_row cs1).
+    induction He1; intros; subst; eauto with kinding.
+  - gen_eq K' : (knd_row cs2).
+    induction He2; intros; subst; eauto with kinding.
+Qed.
+
+Lemma type_equal_variant : forall E T1 T1' T2 T2' K,
+      type_equal E T1 T1' (knd_row cons_universe) ->
+      type_equal E T2 T2' (knd_row cons_universe) ->
+      K = knd_type ->
+      type_equal E (typ_variant T1 T2) (typ_variant T1' T2') K.
+Proof.
+  introv He1 He2 Hkeq.
+  apply type_equal_trans with (typ_variant T1' T2).
+  - gen_eq K' : (knd_row cons_universe).
+    induction He1; intros; subst; eauto with kinding.
+  - gen_eq K' : (knd_row cons_universe).
+    induction He2; intros; subst; eauto with kinding.
+Qed.
+
+Lemma type_equal_arrow : forall E T1 T1' T2 T2' K,
+      type_equal E T1 T1' knd_type ->
+      type_equal E T2 T2' knd_type ->
+      K = knd_type ->
+      type_equal E (typ_arrow T1 T2) (typ_arrow T1' T2') K.
+Proof.
+  introv He1 He2 Hkeq.
+  apply type_equal_trans with (typ_arrow T1' T2).
+  - gen_eq K' : knd_type.
+    induction He1; intros; subst; eauto with kinding.
+  - gen_eq K' : knd_type.
+    induction He2; intros; subst; eauto with kinding.
+Qed.
+
+Lemma type_equal_meet : forall E T1 T1' T2 T2' K,
+      type_equal E T1 T1' K ->
+      type_equal E T2 T2' K ->
+      is_row_kind K ->
+      type_equal E (typ_meet T1 T2) (typ_meet T1' T2') K.
+Proof.
+  introv He1 He2 Hkeq.
+  apply type_equal_trans with (typ_meet T1' T2).
+  - induction He1; intros; subst; eauto with kinding.
+  - induction He2; intros; subst; eauto with kinding.
+Qed.
+
+Lemma type_equal_join : forall E T1 T1' T2 T2' K,
+      type_equal E T1 T1' K ->
+      type_equal E T2 T2' K ->
+      is_row_kind K ->
+      type_equal E (typ_join T1 T2) (typ_join T1' T2') K.
+Proof.
+  introv He1 He2 Hkeq.
+  apply type_equal_trans with (typ_join T1' T2).
+  - induction He1; intros; subst; eauto with kinding.
+  - induction He2; intros; subst; eauto with kinding.
+Qed.
+
+(* *************************************************************** *)
+(** Idempotence of join and meet *)
+
+Lemma type_equal_join_idempotent : forall E T cs,
+    kinding E T (knd_row cs) ->
+    type_equal E (typ_join T T) T (knd_row cs).
+Proof.
+  introv Hk.
+  eapply type_equal_step_l
+    with (typ_join T (typ_meet T (typ_top cs))).
+  - eauto 8 with kinding.
+  - eapply type_equal_single_r; eauto 10 with kinding.
+Qed.    
+
+Lemma type_equal_meet_idempotent : forall E T cs,
+    kinding E T (knd_row cs) ->
+    type_equal E (typ_meet T T) T (knd_row cs).
+Proof.
+  introv Hk.
+  eapply type_equal_step_l
+    with (typ_meet T (typ_join T (typ_bot cs))).
+  - eauto 8 with kinding.
+  - eapply type_equal_single_r; eauto 10 with kinding.
+Qed.
+
+Hint Resolve type_equal_join_idempotent.
+Hint Resolve type_equal_meet_idempotent.
+
+(* *************************************************************** *)
+(** Not affected by type bindings *)
+
+Lemma type_equal_step_bind_typ : forall E F T1 T2 x S,
+    type_equal_step (E & x ~: S & F) T1 T2 ->
+    type_equal_step (E & F) T1 T2.
+Proof.
+  introv Hs.
+  gen_eq G : (E & x ~: S & F).
+  induction Hs; intros; subst; eauto with bind_typ.
+Qed.  
+
+Lemma type_equal_bind_typ : forall E F T1 T2 K x S,
+    type_equal (E & x ~: S & F) T1 T2 K ->
+    type_equal (E & F) T1 T2 K.
+Proof.
+  introv He.
+  gen_eq G : (E & x ~: S & F).
+  induction He; intros; subst;
+    eauto using type_equal_step_bind_typ with bind_typ.
+Qed.  
+
+(* *************************************************************** *)
+(** Preserved by type substitution *)
+
+Lemma type_equal_step_typ_subst : forall E F X T1 T2 S J,
+  type_equal_step (E & X ~:: J & F) T1 T2 -> 
+  kinding E S J -> 
+  type_equal_step (E & (environment_subst X S F))
+             (typ_subst X S T1) (typ_subst X S T2).
+Proof.
+  introv Hs Hk.
+  gen_eq G: (E & X ~:: J & F).
+  induction Hs; intros; subst; simpl typ_subst; auto;
+    do 2 match goal with
+    | H : kinding (E & X ~:: J & F) ?T1 _ |- _ =>
+      apply kinding_typ_subst with (T := T1) (E := E) (S := S) in H
+    end;
+    eauto.
+Qed.
+
+Hint Resolve type_equal_step_typ_subst : typ_subst.
+
+Lemma type_equal_typ_subst : forall E F X T1 T2 S K J,
+  type_equal (E & X ~:: J & F) T1 T2 K -> 
+  kinding E S J -> 
+  type_equal (E & (environment_subst X S F))
+             (typ_subst X S T1) (typ_subst X S T2) K.
+Proof.
+  introv Hkt Hks.
+  gen_eq G: (E & X ~:: J & F).
+  inductions Hkt; intros; subst; eauto with typ_subst.
+Qed.
+
+Hint Resolve type_equal_typ_subst : typ_subst.
+
+(* *************************************************************** *)
+(** Weakening *)
+
+Lemma type_equal_step_weakening : forall E F G T1 T2,
+   type_equal_step (E & G) T1 T2 -> 
+   environment (E & F & G) ->
+   type_equal_step (E & F & G) T1 T2.
+Proof.
+  introv Hs Henv.
+  gen_eq D: (E & G).
+  induction Hs; intros; subst; eauto with weaken.
+Qed.
+
+Hint Resolve type_equal_step_weakening : weaken.
+
+Lemma type_equal_weakening : forall E F G T1 T2 K,
+   type_equal (E & G) T1 T2 K -> 
+   environment (E & F & G) ->
+   type_equal (E & F & G) T1 T2 K.
+Proof.
+  introv Heq Henv.
+  gen_eq D: (E & G).
+  induction Heq; intros; subst; eauto with weaken.
+Qed.
+
+Hint Resolve type_equal_weakening : weaken.
+
+(* *************************************************************** *)
+(** Kind can be replaced *)
+
+Lemma type_equal_replace_kind : forall E T1 T2 K1 K2,
+    kinding E T1 K1 ->
+    type_equal E T1 T2 K2 ->
+    type_equal E T1 T2 K1.
+Proof.
+  introv Hk He.
+  replace K1 with K2
+    by eauto using kinding_unique with kinding.
+  assumption.
+Qed.    
+
+(* *************************************************************** *)
+(** * Properties of Subtyping *)
+
+(* *************************************************************** *)
+(** Reflexivity *)
+
+Lemma subtype_refl : forall E T,
+  kinding E T (knd_row cons_universe) -> 
+  subtype E T T.
+Proof.
+  introv Hk.
+  unfold subtype; auto using type_equal_symm.
+Qed.
+
+(* *************************************************************** *)
+(** Transitivity *)
+
+Lemma subtype_trans : forall E T1 T2 T3,
+    subtype E T1 T2 ->
+    subtype E T2 T3 ->
+    subtype E T1 T3.
+Proof.
+  introv H12 H23.
+  unfold subtype in *.
+  assert (kinding E T1 (knd_row cons_universe))
+    by eauto with kinding.
+  assert (kinding E T2 (knd_row cons_universe))
+    by eauto with kinding.
+  assert (kinding E T3 (knd_row cons_universe)).
+  { assert (kinding E (typ_meet T2 T3) (knd_row cons_universe))
+      as Hk by eauto with kinding.
+    inversion Hk; subst.
+    inversion H7; subst.
+    auto. }
+  apply type_equal_trans with (typ_meet T1 T2); auto.
+  apply type_equal_trans with (typ_meet T1 (typ_meet T2 T3));
+    eauto using type_equal_meet.
+  apply type_equal_trans with (typ_meet (typ_meet T1 T2) T3);
+    eauto using type_equal_single_l with kinding.
+  eauto 6 using type_equal_meet, type_equal_symm.
+Qed.
+
+(* *************************************************************** *)
+(** Anti-symmetry *)
+
+Lemma subtype_antisymm : forall E T1 T2,
+    subtype E T1 T2 ->
+    subtype E T2 T1 ->
+    type_equal E T1 T2 (knd_row cons_universe).
+Proof.
+  introv H12 H21.
+  unfold subtype in *.
+  apply type_equal_trans with (typ_meet T1 T2); auto.
+  apply type_equal_trans with (typ_meet T2 T1);
+    auto using type_equal_symm.
+  eauto with kinding.
+Qed.
+
+(* *************************************************************** *)
+(* Well-kindedness *)
+
+Lemma subtype_kinding : forall E T1 T2,
+    subtype E T1 T2 ->
+    kinding E T1 (knd_row cons_universe)
+    /\ kinding E T2 (knd_row cons_universe).
+Proof.
+  introv He.
+  destruct (type_equal_kinding He) as [ Hk Hj ].
+  split; auto.
+  inversion Hj; subst.
+  inversion H5; subst.
+  auto.
+Qed.
+
+Hint Extern 1 (kinding ?E ?T (knd_row cons_universe)) =>
+  match goal with
+  | H: subtype E T _ |- _ =>
+      apply (proj1 (subtype_kinding H))
+  | H: subtype E _ T |- _ =>
+      apply (proj2 (subtype_kinding H))
+  end : kinding.
+
+(* *************************************************************** *)
+(** Weakening *)
+
+Lemma subtype_weakening : forall E F G T1 T2,
+   subtype (E & G) T1 T2 -> 
+   environment (E & F & G) ->
+   subtype (E & F & G) T1 T2.
+Proof.
+  introv Hs He.
+  apply type_equal_weakening; auto.
+Qed.
+
+Hint Resolve subtype_weakening : weaken.
+
+(* *************************************************************** *)
+(** Not affected by type bindings *)
+
+Lemma subtype_bind_typ : forall E F T1 T2 x S,
+    subtype (E & x ~: S & F) T1 T2 ->
+    subtype (E & F) T1 T2.
+Proof.
+  unfold subtype.
+  introv He.
+  eapply type_equal_bind_typ.
+  apply He.
+Qed.  
+
+Hint Resolve subtype_bind_typ : bind_typ.
+
+(* *************************************************************** *)
+(** Preserved by type substitution *)
+
+Lemma subtype_typ_subst : forall E F X T1 T2 S J,
+  subtype (E & X ~:: J & F) T1 T2 -> 
+  kinding E S J -> 
+  subtype (E & (environment_subst X S F))
+          (typ_subst X S T1) (typ_subst X S T2).
+Proof.
+  unfold subtype.
+  introv Hs Hk.
+  lets H : (type_equal_typ_subst Hs Hk).
+  simpl in H.
+  auto.
+Qed.
+
+Hint Resolve subtype_typ_subst : typ_subst.
+
+(* *************************************************************** *)
+(* Let's try projection as a function *)
+(*
+Fixpoint projection (env : env) (cs : constructors) (t : typ)
+  : option (option typ) :=
+  match t with
+  | typ_bvar _ => None
+  | typ_fvar v =>
+      match EnvOps.get v env with
+      | None => None
+      | Some (bind_typ _) => None
+      | Some (bind_knd knd_type) => None
+      | Some (bind_knd (knd_row cs')) =>
+          match cons_subset cs' cs with
+          | True => Some (Some t)
+          | False =>
+            let cs'' := cons_inter cs cs' in
+            match cons_non_empty cs'' with
+            | True => None
+            | False => Some None
+            end
+          end
+      end
+  | typ_constructor c _ =>
+      match mem c cs with
+      | True => Some (Some t)
+      | _ => Some None
+      end
+  | typ_or t1 t2 =>
+      match projection t1, projection t2 with
+      | Some (Some p1), Some (Some p2) => Some (Some (typ_or p1 p2))
+      | Some (Some p), Some None => Some (Some p)
+      | Some None, Some (Some p) => Some (Some p)
+      | Some None, Some None => Some None
+      | _, _ => None
+      end
+  | typ_variant _ _ => None
+  | typ_arrow _ _ => None
+  | typ_top cs' =>
+      let cs'' := cons_inter cs cs' in
+      match cons_non_empty cs'' with
+      | True => Some (Some (typ_top cs''))
+      | False => Some None
+      end
+  | typ_bot cs' =>
+      let cs'' := cons_inter cs cs' in
+      match cons_non_empty cs'' with
+      | True => Some (Some (typ_bot cs''))
+      | False => Some None
+      end
+  | typ_meet t1 t2 =>
+      match projection t1, projection t2 with
+      | Some (Some p1), Some (Some p2) => Some (Some (typ_meet p1 p2))
+      | Some None, Some None => Some None
+      | _, _ => None
+      end
+  | typ_join t1 t2 =>
+      match projection t1, projection t2 with
+      | Some (Some p1), Some (Some p2) => Some (Some (typ_join p1 p2))
+      | Some None, Some None => Some None
+      | _, _ => None
+      end
+  end.
+*)
+
+(* *************************************************************** *)
+(** TODO: Describe and rename these lemmas *)
+
+Inductive row_projection : env -> typ -> constructors ->
+                           typ -> constructors -> Prop :=
+  | row_projection_var : forall E cs X,
+      row_projection E (typ_fvar X) cs (typ_fvar X) cs
+  | row_projection_constructor : forall E c cs T,
+      row_projection E (typ_constructor c T) cs
+                       (typ_constructor c T) cs
+  | row_projection_or : forall E cs1 cs2 cs3 cs4 T1 T2 T,
+      kinding E T1 (knd_row cs3) ->
+      kinding E T2 (knd_row cs4) ->
+      or_projection E T1 cs3 T2 cs4 T cs1 ->
+      row_projection E (typ_or T1 T2) cs2 T cs1
+  | row_projection_meet : forall E cs1 cs2 T1 T2 T3 T4,
+      row_projection E T1 cs2 T3 cs1 ->
+      row_projection E T2 cs2 T4 cs1 ->
+      row_projection E (typ_meet T1 T2) cs2 (typ_meet T3 T4) cs1
+  | row_projection_join : forall E cs1 cs2 T1 T2 T3 T4,
+      row_projection E T1 cs2 T3 cs1 ->
+      row_projection E T2 cs2 T4 cs1 ->
+      row_projection E (typ_join T1 T2) cs2 (typ_join T3 T4) cs1
+  | row_projection_bot : forall E cs1 cs2,
+      kinding E (typ_bot cs1) (knd_row cs1) ->
+      cons_subset cs1 cs2 ->
+      row_projection E (typ_bot cs2) cs2 (typ_bot cs1) cs1
+  | row_projection_top : forall E cs1 cs2,
+      kinding E (typ_top cs1) (knd_row cs1) ->
+      cons_subset cs1 cs2 ->
+      row_projection E (typ_top cs2) cs2 (typ_top cs1) cs1
+
+with or_projection : env ->
+                     typ -> constructors ->
+                     typ -> constructors ->
+                     typ -> constructors -> Prop :=
+  | or_left : forall E T1 cs1 T2 cs2 T cs,
+      cons_subset cs cs1 ->
+      row_projection E T1 cs1 T cs ->
+      or_projection E T1 cs1 T2 cs2 T cs
+  | or_right : forall E T1 cs1 T2 cs2 T cs,
+      cons_subset cs cs2 ->
+      row_projection E T2 cs2 T cs ->
+      or_projection E T1 cs1 T2 cs2 T cs
+  | or_both : forall E T1 cs1 T2 cs2 T1' T2' cs,
+      cons_non_empty (cons_inter cs cs1) ->
+      cons_non_empty (cons_inter cs cs2) ->
+      cs = (cons_union (cons_inter cs cs1) (cons_inter cs cs2)) ->
+      row_projection E T1 cs1 T1' (cons_inter cs cs1) ->
+      row_projection E T2 cs2 T2' (cons_inter cs cs2) ->
+      or_projection E T1 cs1 T2 cs2 (typ_or T1' T2') cs.
+
+Hint Constructors row_projection or_projection.
+
+Scheme row_projection_mut := Induction for row_projection Sort Prop
+  with or_projection_mut := Induction for or_projection Sort Prop.
+
+Combined Scheme projection_mut from
+         row_projection_mut, or_projection_mut.
+
+Lemma row_projection_identity_ind : forall E cs1 cs2 T,
+    kinding E T (knd_row cs1) ->
+    cs1 = cs2 ->
+    row_projection E T cs1 T cs2.
+Proof.
+  introv Hk.
+  gen_eq K : (knd_row cs1).
+  gen cs1 cs2.
+  induction Hk; introv Hknd Heq; subst; auto;
+    inversion Hknd; subst; auto;
+    invert_kind; eauto with constrs.
+Qed.    
+
+Lemma row_projection_identity : forall E cs T,
+    kinding E T (knd_row cs) ->
+    row_projection E T cs T cs.
+Proof.
+  introv Hknd.
+  apply row_projection_identity_ind; auto.
+Qed.
+
+Lemma row_projection_kinding_mut :
+    (forall E T cs T' cs',
+    kinding E T (knd_row cs) ->
+    row_projection E T cs T' cs' ->
+    kinding E T' (knd_row cs'))
+/\ (forall E T1 cs1 T2 cs2 T' cs',
+    kinding E T1 (knd_row cs1) ->
+    kinding E T2 (knd_row cs2) ->
+    kinding E (typ_or T1 T2) (knd_row (cons_union cs1 cs2)) ->
+    or_projection E T1 cs1 T2 cs2 T' cs' ->
+    kinding E T' (knd_row cs')).
+Proof.
+  apply projection_mut; intros; substs; intuition auto with constrs.
+  - rewrite e.
+    auto with constrs.
+Qed.
+
+Definition row_projection_kinding :=
+  proj1 row_projection_kinding_mut.
+
+Hint Resolve row_projection_kinding.
+
+Lemma row_projection_idem : forall E cs T T',
+    row_projection E T (knd_row cs) cs T' ->
+    T = T'.
+Proof.
+  introv Hpr.
+  gen_eq K : (knd_row cs).
+  induction Hpr; intro; auto.
+  - assert (cons_non_empty cs3) by auto.
+    apply row_projection_kinding in Hpr.
+    assert (cons_non_empty cs2) by iauto.
+    inversion H2; subst.
+    false.
+    constrs.
+  - assert (cons_non_empty cs2) by auto.
+    apply row_projection_kinding in Hpr.
+    assert (cons_non_empty cs3) by iauto.
+    inversion H2; subst.
+    false.
+    constrs.
+  - inversion H3; subst.
+    replace T1' with T1
+      by auto with constrs.
+    replace T2' with T2
+      by auto with constrs.
+    auto.
+  - replace T3 with T1 by auto.
+    replace T4 with T2 by auto.
+    auto.
+  - replace T3 with T1 by auto.
+    replace T4 with T2 by auto.
+    auto.
+  - inversion H2.
+    auto.
+  - inversion H2.
+    auto.
+Qed.
+
+Ltac equal_kinds :=
+  repeat
+    match goal with
+    | [ Hr : row_projection ?E ?T (knd_row ?cs) _ _ |- _ ] =>
+      match goal with
+      | [ Hk : kinding E T (knd_row cs) |- _ ] =>
+        fail 1
+      | _ =>
+        let Hk := fresh "Hk" in
+        assert (kinding E T (knd_row cs)) as Hk
+            by (apply (proj1 (row_projection_kinding Hr)))
+      end
+    | [ He : type_equal ?E ?T _ (knd_row ?cs) |- _ ] =>
+      match goal with
+      | [ Hk : kinding E T (knd_row cs) |- _ ] =>
+        fail 1
+      | _ =>
+        let Hk := fresh "Hk" in
+        assert (kinding E T (knd_row cs)) as Hk
+            by (apply (proj1 (type_equal_kinding He)))
+      end
+    | [ He : type_equal ?E _ ?T (knd_row ?cs) |- _ ] =>
+      match goal with
+      | [ Hk : kinding E T (knd_row cs) |- _ ] =>
+        fail 1
+      | _ =>
+        let Hk := fresh "Hk" in
+        assert (kinding E T (knd_row cs)) as Hk
+            by (apply (proj2 (type_equal_kinding He)))
+      end
+    end;
+  repeat
+    match goal with
+    | [ Hk1 : kinding ?E ?T (knd_row ?cs1),
+        Hk2 : kinding ?E ?T (knd_row ?cs2) |- _ ] =>
+      match goal with
+      | [ Heq : (knd_row cs1) = (knd_row cs2) |- _ ] =>
+        fail 1
+      | [ Heq : (knd_row cs2) = (knd_row cs1) |- _ ] =>
+        fail 1
+      | _ =>
+        let Heq := fresh "Heq" in
+        assert ((knd_row cs1) = (knd_row cs2)) as Heq
+            by apply (kinding_unique Hk1 Hk2);
+        inversion Heq;
+        clear Heq;
+        clear Hk2
+      end
+    end;
+  substs.
+
+Lemma row_projection_unique : forall E cs T K T' T'',
+    row_projection E T K cs T' ->
+    row_projection E T K cs T'' ->
+    T' = T''.
+Proof.
+  introv Hpr1 Hpr2.
+  gen T''.
+  induction Hpr1; introv Hpr2.
+  - eauto using row_projection_idem.
+  - inversion Hpr2; subst; equal_kinds; auto.
+    + assert (cons_non_empty cs3) by auto.
+      false.
+      constrs.
+    + assert (cons_non_empty cs1).
+      { apply row_projection_kinding in Hpr1.
+        iauto. }
+      false.
+      constrs.
+    + false.
+      constrs.
+  - inversion Hpr2; subst; equal_kinds; auto.
+    + assert (cons_non_empty cs2) by auto.
+      false.
+      constrs.
+    + assert (cons_non_empty cs1).
+      { apply row_projection_kinding in Hpr1.
+        iauto. }
+      false.
+      constrs.
+    + false.
+      constrs.
+  - inversion Hpr2; subst.
+    + replace (cons_inter (cons_union cs2 cs3) cs2)
+        with cs2 in Hpr1_1 by constrs.
+      replace (cons_inter (cons_union cs2 cs3) cs3)
+        with cs3 in Hpr1_2 by constrs.
+      apply row_projection_idem in Hpr1_1.
+      apply row_projection_idem in Hpr1_2.
+      subst.
+      reflexivity.
+    + equal_kinds.
+      false.
+      constrs.
+    + equal_kinds.
+      false.
+      constrs.
+    + equal_kinds.
+      f_equal; auto.
+  - inversion Hpr2; subst.
+    + apply row_projection_idem in Hpr1_1.
+      apply row_projection_idem in Hpr1_2.
+      subst.
+      reflexivity.
+    + f_equal; auto.
+  - inversion Hpr2; subst.
+    + apply row_projection_idem in Hpr1_1.
+      apply row_projection_idem in Hpr1_2.
+      subst.
+      reflexivity.
+    + f_equal; auto.
+  - inversion Hpr2; subst; auto.
+  - inversion Hpr2; subst; auto.
+Qed.
+
+Lemma type_equal_project : forall E cs T1 T2 T1' K,
+    type_equal E T1 T2 K ->
+    row_projection E T1 K cs T1' ->
+    exists T2',
+    row_projection E T2 K cs T2' /\
+    type_equal E T1' T2' (knd_row cs).
+Proof.
+  introv He Hpr.
+  gen T1' cs.
+  induction He; introv Hpr.
+  - eauto using type_equal_refl with kinding.
+  - inversion Hpr; subst.
+    exists (typ_constructor c T').
+    auto with kinding.
+  - inversion Hpr; subst.
+    + exists (typ_or T1' T2').
+      auto with kinding.
+    + equal_kinds.
+      destruct (IHHe1 _ _ H6) as [T1'' ?].
+      exists T1''.
+      iauto.
+    + equal_kinds.
+      destruct (IHHe2 _ _ H9) as [T2'' ?].
+      exists T2''.
+      iauto.
+    + equal_kinds.
+      destruct (IHHe1 _ _ H8) as [T1'' ?].
+      destruct (IHHe2 _ _ H11) as [T2'' ?].
+      exists (typ_or T1'' T2'').
+      split; iauto.
+      replace cs
+        with (cons_union (cons_inter cs cs1) (cons_inter cs cs2))
+        by constrs.
+      intuition auto with constrs.
+  - inversion Hpr.
+  - inversion Hpr.
+  - inversion Hpr; subst; eauto with kinding.
+  - inversion Hpr; subst; eauto with kinding.
+  - inversion Hpr; subst.
+    + exists (typ_meet T1' T2').
+      auto with kinding.
+    + destruct (IHHe1 _ _ H2) as [T1'' ?].
+      destruct (IHHe2 _ _ H6) as [T2'' ?].
+      exists (typ_meet T1'' T2'').
+      iauto.
+  - inversion Hpr; subst.
+    + exists (typ_join T1' T2').
+      auto with kinding.
+    + destruct (IHHe1 _ _ H2) as [T1'' ?].
+      destruct (IHHe2 _ _ H6) as [T2'' ?].
+      exists (typ_join T1'' T2'').
+      iauto.
+  - destruct (IHHe1 _ _ Hpr) as [T2' [Hpr2 ?]].
+    destruct (IHHe2 _ _ Hpr2) as [T3' ?].
+    iauto.
+  - replace (cons_union cs1 cs2)
+        with (cons_union cs2 cs1) in * by constrs.
+    assert (cons_disjoint cs2 cs1) by constrs.
+    inversion Hpr; subst.
+    + exists (typ_or T2 T1).
+      intuition auto using type_equal_symm.
+    + equal_kinds.
+      exists T1'.
+      replace (cons_union cs3 cs4)
+        with (cons_union cs4 cs3) in * by constrs.
+      auto using type_equal_refl with kinding.
+    + equal_kinds.
+      exists T1'.
+      replace (cons_union cs3 cs4)
+        with (cons_union cs4 cs3) in * by constrs.
+      auto using type_equal_refl with kinding.
+    + equal_kinds.
+      exists (typ_or T2' T1'0).
+      replace (cons_union cs3 cs4)
+        with (cons_union cs4 cs3) in * by constrs.
+      split; auto.
+      replace cs
+        with (cons_union (cons_inter cs cs3) (cons_inter cs cs4))
+        by constrs.
+      auto with kinding constrs.
+  - inversion Hpr; subst.
+    + exists (typ_or (typ_or T1 T2) T3).
+      split; auto.
+      rewrite cons_union_associative.
+      auto with constrs.
+    + assert (kinding E (typ_or T2 T3) (knd_row (cons_union cs2 cs3)))
+        by auto.
+      equal_kinds.
+      exists T1'.
+      split; auto using type_equal_refl with kinding.
+      rewrite cons_union_associative.
+      apply row_projection_or_l; auto with kinding; constrs.
+    + { inversion H14; subst.
+        - assert
+            (kinding E (typ_or T2 T3) (knd_row (cons_union cs2 cs3)))
+            by auto.
+          equal_kinds.
+          assert (cons_non_empty cs2) by auto.
+          assert (cons_non_empty cs3) by auto.
+          exists (typ_or T2 T3).
+          split; auto using type_equal_refl with kinding.
+          rewrite cons_union_associative.
+          apply row_projection_or_both; auto with constrs.
+          + replace (cons_inter (cons_union cs2 cs3)
+                                (cons_union cs4 cs2))
+              with cs2 by constrs.
+            apply row_projection_or_r; auto; constrs.
+          + replace (cons_inter (cons_union cs2 cs3) cs3)
+              with cs3 by constrs.
+            apply row_projection_identity.
+            auto with kinding.
+        - equal_kinds.
+          exists T1'.
+          split; auto using type_equal_refl with kinding.
+          rewrite cons_union_associative.
+          apply row_projection_or_l; auto; constrs.
+        - equal_kinds.
+          exists T1'.
+          split; auto using type_equal_refl with kinding.
+          rewrite cons_union_associative.
+          apply row_projection_or_r; auto; constrs.
+        - equal_kinds.
+          exists (typ_or T1'0 T2').
+          split; auto using type_equal_refl with kinding.
+          rewrite cons_union_associative.
+          apply row_projection_or_both; auto with constrs.
+          apply row_projection_or_r; auto with constrs.
+          replace (cons_inter cs (cons_union cs4 cs6))
+            with (cons_inter cs cs6) by constrs.
+          auto. }
+      + { inversion H16; substs.
+          - assert
+              (kinding E (typ_or T2 T3)
+                       (knd_row (cons_union cs2 cs3)))
+              by auto.
+            rewrite <- H15 in H14.
+            equal_kinds.
+            exists (typ_or (typ_or T1'0 T2) T3).
+            split.
+            + { rewrite <- H15.
+                rewrite cons_union_associative.
+                apply row_projection_or_both.
+                - constrs.
+                - constrs.
+                - constrs.
+
+            + assert
+                (kinding E (typ_or T1'0 (typ_or T2 T3)) (knd_row cs))
+                by auto with kinding.
+              assert
+                (kinding E (typ_or T1'0 (typ_or T2 T3))
+                         (knd_row (cons_union (cons_inter cs cs4)
+                                              (cons_union cs2 cs3)))).
+              { apply row_projection_kinding in H13.
+                apply kinding_or; auto with constrs. }
+              equal_kinds.
+              apply type_equal_or_associative_l;
+                auto with constrs kinding.
