Makefile
@@ -1,0 +1,16 @@
+
+COQC=coqc
+COQPARAMS=-R ~/Repositories/tlc/src TLC
+
+MODULES=Cofinite.vo Definitions.vo Infrastructure.vo Kinding.vo
+
+all: ${MODULES}
+
+%.vo: %.v
+	${COQC} ${COQPARAMS} $<
+
+Infrastructure.vo: Definitions.vo
+Kinding.vo: Definitions.vo Infrastructure.vo
+
+clean:
+	@rm -f *.vo *.glob .*.aux
